Fsub/Fsub_LetSum_Infrastructure.v
@@ -20,6 +20,8 @@
       - #<a href="##body">Properties of body_e</a># *)
 
 Require Export Fsub.Fsub_LetSum_Definitions.
+Require Import Coq.Logic.Decidable.
+Require Import Coq.Bool.Bool.
 
 
 (* ********************************************************************** *)
@@ -33,42 +35,90 @@ Require Export Fsub.Fsub_LetSum_Definitions.
     straightforward since bound variables are indices, not names, in
     locally nameless representation. *)
 
-Fixpoint fv_tt (T : typ) {struct T} : atoms :=
-  match T with
-  | typ_top => {}
-  | typ_bvar J => {}
-  | typ_fvar X => {{ X }}
-  | typ_arrow T1 T2 => (fv_tt T1) `union` (fv_tt T2)
-  | typ_all T1 T2 => (fv_tt T1) `union` (fv_tt T2)
-  | typ_sum T1 T2 => (fv_tt T1) `union` (fv_tt T2)
-  end.
+(* Note, the only purpose of this function is the avoid naming conflicts, 
+   as a result, this stupid definition below works *)
 
-Fixpoint fv_te (e : exp) {struct e} : atoms :=
+Definition fv_cc (C : captureset): atoms :=
+  match C with
+  | cset_universal => {}
+  | cset_set As Ns => As 
+  end
+.
+
+
+Definition fv_ec (C : captureset): atoms :=
+  match C with
+  | cset_universal => {}
+  | cset_set As Ns => As
+  end
+.
+
+Fixpoint fv_ss (Sh : shp) {struct Sh} : atoms :=
+  match Sh with
+  | shp_top => {}
+  | shp_bvar J => {}
+  | shp_fvar X => {{ X }}
+  | shp_arrow T1 T2 => (fv_st T1) `union` (fv_st T2)
+  | shp_sall Sh1 T => (fv_ss Sh1) `union` (fv_st T)
+  | shp_call C T => (fv_st T)
+  end
+with fv_st (T : typ) {struct T} : atoms :=
+  match T with
+  | pair Sh1 C => (fv_ss Sh1) 
+  end
+.
+
+Fixpoint fv_cs (Sh : shp) {struct Sh} : atoms :=
+  match Sh with
+  | shp_top => {}
+  | shp_bvar J => {}
+  | shp_fvar X => {}
+  | shp_arrow T1 T2 => (fv_ct T1) `union` (fv_ct T2)
+  | shp_sall Sh1 T => (fv_cs Sh1) `union` (fv_ct T)
+  | shp_call C T => (fv_cc C) `union` (fv_ct T)
+  end
+with fv_ct (T : typ) {struct T} : atoms :=
+  match T with
+  | pair Sh1 C => (fv_cs Sh1) `union` (fv_cc C)
+  end
+.
+
+Fixpoint fv_se (e : exp) {struct e} : atoms :=
   match e with
   | exp_bvar i => {}
   | exp_fvar x => {}
-  | exp_abs V e1  => (fv_tt V) `union` (fv_te e1)
-  | exp_app e1 e2 => (fv_te e1) `union` (fv_te e2)
-  | exp_tabs V e1 => (fv_tt V) `union` (fv_te e1)
-  | exp_tapp e1 V => (fv_tt V) `union` (fv_te e1)
-  | exp_let e1 e2 => (fv_te e1) `union` (fv_te e2)
-  | exp_inl e1 => (fv_te e1)
-  | exp_inr e1 => (fv_te e1)
-  | exp_case e1 e2 e3 => (fv_te e1) `union` (fv_te e2) `union` (fv_te e3)
-  end.
+  | exp_abs V e1  => (fv_st V) `union` (fv_se e1)
+  | exp_app e1 C e2 => (fv_se e1) `union` (fv_se e2)
+  | exp_sabs V e1 => (fv_ss V) `union` (fv_se e1)
+  | exp_sapp e1 V => (fv_ss V) `union` (fv_se e1)
+  | exp_cabs C e1 => (fv_se e1)
+  | exp_capp e1 C => (fv_se e1)
+  end
+.
+
+Fixpoint fv_ce (e : exp) {struct e} : atoms :=
+  match e with
+  | exp_bvar i => {}
+  | exp_fvar x => {}
+  | exp_abs V e1  => (fv_ct V) `union` (fv_ce e1)
+  | exp_app e1 C e2 => (fv_ce e1) `union` (fv_cc C) `union` (fv_ce e2)
+  | exp_sabs V e1 => (fv_cs V) `union` (fv_ce e1)
+  | exp_sapp e1 V => (fv_cs V) `union` (fv_ce e1)
+  | exp_cabs C e1 => (fv_cc C) `union` (fv_ce e1)
+  | exp_capp e1 C => (fv_cc C) `union` (fv_ce e1)
+  end
+.
 
 Fixpoint fv_ee (e : exp) {struct e} : atoms :=
   match e with
   | exp_bvar i => {}
   | exp_fvar x => {{ x }}
   | exp_abs V e1 => (fv_ee e1)
-  | exp_app e1 e2 => (fv_ee e1) `union` (fv_ee e2)
-  | exp_tabs V e1 => (fv_ee e1)
-  | exp_tapp e1 V => (fv_ee e1)
-  | exp_let e1 e2 => (fv_ee e1) `union` (fv_ee e2)
-  | exp_inl e1 => (fv_ee e1)
-  | exp_inr e1 => (fv_ee e1)
-  | exp_case e1 e2 e3 => (fv_ee e1) `union` (fv_ee e2) `union` (fv_ee e3)
+  | exp_app e1 C e2 => (fv_ee e1) `union` (fv_ec C) `union` (fv_ee e2)
+  | exp_sabs V e1 => (fv_ee e1)
+  | exp_sapp e1 V => (fv_ee e1)
+  | exp_cabs V e1 => (fv_ee e1)
+  | exp_capp e1 V => (fv_ee e1)
   end.
 
 
@@ -88,52 +138,101 @@ Fixpoint fv_ee (e : exp) {struct e} : atoms :=
         closed.  Thus, there is no need to shift indices when passing
         under a binder. *)
 
-Fixpoint subst_tt (Z : atom) (U : typ) (T : typ) {struct T} : typ :=
+Fixpoint subst_ss (Z : atom) (U : shp) (T : shp) {struct T} : shp :=
   match T with
-  | typ_top => typ_top
-  | typ_bvar J => typ_bvar J
-  | typ_fvar X => if X == Z then U else T
-  | typ_arrow T1 T2 => typ_arrow (subst_tt Z U T1) (subst_tt Z U T2)
-  | typ_all T1 T2 => typ_all (subst_tt Z U T1) (subst_tt Z U T2)
-  | typ_sum T1 T2 => typ_sum (subst_tt Z U T1) (subst_tt Z U T2)
-  end.
+  | shp_top => shp_top
+  | shp_bvar J => shp_bvar J
+  | shp_fvar X => if X == Z then U else T
+  | shp_arrow T1 T2 => shp_arrow (subst_st Z U T1) (subst_st Z U T2)
+  | shp_sall Sh T2 => shp_sall (subst_ss Z U Sh) (subst_st Z U T2)
+  | shp_call C T2 => shp_call C (subst_st Z U T2)
+  end
+with subst_st (Z : atom) (U : shp) (T : typ) {struct T}: typ :=
+  match T with
+  | pair Sh C => pair (subst_ss Z U Sh) C
+  end
+.
 
-Fixpoint subst_te (Z : atom) (U : typ) (e : exp) {struct e} : exp :=
+Fixpoint subst_se (Z : atom) (U : shp) (e : exp) {struct e} : exp :=
   match e with
   | exp_bvar i => exp_bvar i
   | exp_fvar x => exp_fvar x
-  | exp_abs V e1 => exp_abs  (subst_tt Z U V)  (subst_te Z U e1)
-  | exp_app e1 e2 => exp_app  (subst_te Z U e1) (subst_te Z U e2)
-  | exp_tabs V e1 => exp_tabs (subst_tt Z U V)  (subst_te Z U e1)
-  | exp_tapp e1 V => exp_tapp (subst_te Z U e1) (subst_tt Z U V)
-  | exp_let e1 e2 => exp_let (subst_te Z U e1) (subst_te Z U e2)
-  | exp_inl e1 => exp_inl (subst_te Z U e1)
-  | exp_inr e1 => exp_inr (subst_te Z U e1)
-  | exp_case e1 e2 e3 => exp_case (subst_te Z U e1)
-                                  (subst_te Z U e2) (subst_te Z U e3)
+  | exp_abs V e1 => exp_abs  (subst_st Z U V)  (subst_se Z U e1)
+  | exp_app e1 C e2 => exp_app (subst_se Z U e1) C (subst_se Z U e2)
+  | exp_sabs V e1 => exp_sabs (subst_ss Z U V)  (subst_se Z U e1)
+  | exp_sapp e1 V => exp_sapp (subst_se Z U e1) (subst_ss Z U V)
+  | exp_cabs V e1 => exp_cabs V (subst_se Z U e1)
+  | exp_capp e1 V => exp_capp (subst_se Z U e1) V
   end.
 
-Fixpoint subst_ee (z : atom) (u : exp) (e : exp) {struct e} : exp :=
+Fixpoint subst_cc (Z : atom) (U : captureset) (C : captureset) {struct C} : captureset :=
+  match C with
+  | cset_universal => cset_universal
+  | cset_set As Ns => match (AtomSetImpl.mem Z As) with
+                      | false => cset_set As Ns
+                      | true => match U with
+                                | cset_universal => cset_universal
+                                | cset_set UAs UNs => cset_set (AtomSetImpl.union (AtomSetImpl.remove Z As) UAs) (NatSetImpl.union Ns UNs)
+                                end
+                      end
+  end
+.
+Arguments  subst_cc : simpl never.
+
+
+Fixpoint subst_cs (Z : atom) (U : captureset) (Sh : shp) {struct Sh} : shp :=
+  match Sh with
+  | shp_top => shp_top
+  | shp_bvar J => shp_bvar J
+  | shp_fvar X => shp_fvar X
+  | shp_arrow T1 T2 => shp_arrow (subst_ct Z U T1) (subst_ct Z U T2)
+  | shp_sall Sh T2 => shp_sall (subst_cs Z U Sh) (subst_ct Z U T2)
+  | shp_call C T2 => shp_call (subst_cc Z U C) (subst_ct Z U T2)
+  end
+with subst_ct (Z : atom) (U : captureset) (T : typ) {struct T} : typ :=
+ match T with
+ | pair Sh C => pair (subst_cs Z U Sh) (subst_cc Z U C)
+ end. 
+
+Fixpoint subst_ce (Z : atom) (U : captureset) (e : exp) {struct e} : exp :=
+  match e with
+  | exp_bvar i => exp_bvar i
+  | exp_fvar x => exp_fvar x
+  | exp_abs V e1 => exp_abs (subst_ct Z U V) (subst_ce Z U e1)
+  | exp_app e1 C e2 => exp_app (subst_ce Z U e1) (subst_cc Z U C) (subst_ce Z U e2)
+  | exp_sabs V e1 => exp_sabs (subst_cs Z U V) (subst_ce Z U e1)
+  | exp_sapp e1 V => exp_sapp (subst_ce Z U e1) (subst_cs Z U V)
+  | exp_cabs C e1 => exp_cabs (subst_cc Z U C) (subst_ce Z U e1)
+  | exp_capp e1 C => exp_capp (subst_ce Z U e1) (subst_cc Z U C)
+  end
+.
+
+Fixpoint subst_ee (z : atom) (U : captureset) (u : exp) (e : exp) {struct e} : exp :=
   match e with
   | exp_bvar i => exp_bvar i
   | exp_fvar x => if x == z then u else e
-  | exp_abs V e1 => exp_abs V (subst_ee z u e1)
-  | exp_app e1 e2 => exp_app (subst_ee z u e1) (subst_ee z u e2)
-  | exp_tabs V e1 => exp_tabs V (subst_ee z u e1)
-  | exp_tapp e1 V => exp_tapp (subst_ee z u e1) V
-  | exp_let e1 e2 => exp_let (subst_ee z u e1) (subst_ee z u e2)
-  | exp_inl e1 => exp_inl (subst_ee z u e1)
-  | exp_inr e1 => exp_inr (subst_ee z u e1)
-  | exp_case e1 e2 e3 => exp_case (subst_ee z u e1)
-                                  (subst_ee z u e2) (subst_ee z u e3)
+  | exp_abs V e1 => exp_abs (subst_ct z U V) (subst_ee z U u e1)
+  | exp_app e1 C e2 => exp_app (subst_ee z U u e1) (subst_cc z U C) (subst_ee z U u e2)
+  | exp_sabs V e1 => exp_sabs (subst_cs z U V) (subst_ee z U u e1)
+  | exp_sapp e1 V => exp_sapp (subst_ee z U u e1) (subst_cs z U V)
+  | exp_cabs V e1 => exp_cabs (subst_cc z U V) (subst_ee z U u e1)
+  | exp_capp e1 V => exp_capp (subst_ee z U u e1) (subst_cc z U V)
   end.
 
-Definition subst_tb (Z : atom) (P : typ) (b : binding) : binding :=
+Definition subst_sb (Z : atom) (P : shp) (b : binding) : binding :=
   match b with
-  | bind_sub T => bind_sub (subst_tt Z P T)
-  | bind_typ T => bind_typ (subst_tt Z P T)
+  | bind_sub_shp Sh => bind_sub_shp (subst_ss Z P Sh)
+  | bind_sub_cap C => bind_sub_cap C
+  | bind_typ T => bind_typ (subst_st Z P T)
   end.
 
+Definition subst_cb (Z : atom) (P : captureset) (b : binding) : binding :=
+  match b with
+  | bind_sub_shp Sh => bind_sub_shp (subst_cs Z P Sh)
+  | bind_sub_cap C => bind_sub_cap (subst_cc Z P C)
+  | bind_typ T => bind_typ (subst_ct Z P T)
+  end
+.
 
 (* ********************************************************************** *)
 (** * #<a name="gather_atoms"></a># The "[gather_atoms]" tactic *)
@@ -158,11 +257,14 @@ Definition subst_tb (Z : atom) (P : typ) (b : binding) : binding :=
 Ltac gather_atoms ::=
   let A := gather_atoms_with (fun x : atoms => x) in
   let B := gather_atoms_with (fun x : atom => singleton x) in
-  let C := gather_atoms_with (fun x : exp => fv_te x) in
-  let D := gather_atoms_with (fun x : exp => fv_ee x) in
-  let E := gather_atoms_with (fun x : typ => fv_tt x) in
-  let F := gather_atoms_with (fun x : env => dom x) in
-  constr:(A `union` B `union` C `union` D `union` E `union` F).
+  let C := gather_atoms_with (fun x : exp => fv_se x) in
+  let D := gather_atoms_with (fun x : exp => fv_ce x) in
+  let E := gather_atoms_with (fun x : exp => fv_ee x) in
+  let F := gather_atoms_with (fun x : typ => fv_st x) in
+  let G := gather_atoms_with (fun x : typ => fv_ct x) in
+  let H := gather_atoms_with (fun x : env => dom x) in
+  let I := gather_atoms_with (fun x : captureset => fv_cc x) in
+  constr:(A `union` B `union` C `union` D `union` E `union` F `union` G `union` H `union` I).
 
 
 (* ********************************************************************** *)
@@ -195,76 +297,649 @@ Ltac gather_atoms ::=
 (* ********************************************************************** *)
 (** ** Properties of type substitution in types *)
 
+(* A few lemmas to make my life easier.  
+   TODO: (Edward) Adopt MetaLib to reintroduce equality on sets *)
+
+Axiom NatSetEqual : forall s1 s2,
+  s1 = s2 <-> NatSetImpl.Equal s1 s2.
+
+Axiom AtomSetEqual : forall s1 s2,
+  s1 = s2 <-> AtomSetImpl.Equal s1 s2.
+
+Definition sumbool_to_or {P : Prop} {Q : Prop} (H : (sumbool P Q)) :=
+  match H with
+    | left p0 => or_introl p0
+    | right q0 => or_intror q0
+  end.
+
+Lemma union_empty_atoms: forall s,
+  s = (AtomSetImpl.union s {}).
+Proof.
+  intro s.
+  apply AtomSetEqual.
+  intro a. split;intro aIn.
+  * apply AtomSetImpl.union_2.
+    apply aIn.
+  * apply AtomSetImpl.union_1 in aIn.
+    destruct aIn.
+    ** apply H.
+    ** destruct (AtomSetImpl.empty_1 H).
+Qed.
+
+Lemma union_empty_nats: forall s,
+  s = (NatSetImpl.union s {}N).
+Proof.
+  intro s.
+  apply NatSetEqual.
+  intro a. split;intro aIn.
+  * apply NatSetImpl.union_2.
+    apply aIn.
+  * apply NatSetImpl.union_1 in aIn.
+    destruct aIn.
+    ** apply H.
+    ** destruct (NatSetImpl.empty_1 H).
+Qed.
+
+Lemma mem_union_or_atoms: forall s T1 T2,
+  AtomSetImpl.mem s (union T1 T2) = 
+  (AtomSetImpl.mem s T1) || (AtomSetImpl.mem s T2).
+Proof with auto.
+  intros s T1 T2.
+  destruct (AtomSetImpl.mem s T1) eqn:sInT1; destruct (AtomSetImpl.mem s T2) eqn:sInT2;simpl.
+  * apply AtomSetImpl.mem_1. apply AtomSetImpl.union_2. apply AtomSetFacts.mem_iff in sInT1...
+  * apply AtomSetImpl.mem_1. apply AtomSetImpl.union_2. apply AtomSetFacts.mem_iff in sInT1...
+  * apply AtomSetImpl.mem_1. apply AtomSetImpl.union_3. apply AtomSetFacts.mem_iff in sInT2...
+  * apply AtomSetFacts.not_mem_iff. intro H. apply AtomSetFacts.union_iff in H. destruct H.
+    ** apply AtomSetFacts.not_mem_iff in sInT1. apply (sInT1 H).
+    ** apply AtomSetFacts.not_mem_iff in sInT2. apply (sInT2 H).
+Qed.
+
+Lemma mem_union_or_nats: forall s T1 T2,
+  NatSetImpl.mem s (NatSetImpl.union T1 T2) = 
+  (NatSetImpl.mem s T1) || (NatSetImpl.mem s T2).
+Proof with auto.
+  intros s T1 T2.
+  destruct (NatSetImpl.mem s T1) eqn:sInT1; destruct (NatSetImpl.mem s T2) eqn:sInT2;simpl.
+  * apply NatSetImpl.mem_1. apply NatSetImpl.union_2. apply NatSetFacts.mem_iff in sInT1...
+  * apply NatSetImpl.mem_1. apply NatSetImpl.union_2. apply NatSetFacts.mem_iff in sInT1...
+  * apply NatSetImpl.mem_1. apply NatSetImpl.union_3. apply NatSetFacts.mem_iff in sInT2...
+  * apply NatSetFacts.not_mem_iff. intro H. apply NatSetFacts.union_iff in H. destruct H.
+    ** apply NatSetFacts.not_mem_iff in sInT1. apply (sInT1 H).
+    ** apply NatSetFacts.not_mem_iff in sInT2. apply (sInT2 H).
+Qed.
+
+
+Lemma cset_subset : forall t t0 t1 t2 C1 C2,
+  C1 = cset_set t t0 ->
+  C2 = cset_set t1 t2 ->
+  (cset_subset_prop C1 C2) ->
+  (AtomSetImpl.Subset t t1) /\ (NatSetImpl.Subset t0 t2).
+Proof with auto.
+  intros T T0 T1 T2 C1 C2 SC1 SC2 H.
+  split; destruct H eqn:shpH...
+  * discriminate SC2.
+  * inversion SC2. inversion SC1.
+    rewrite <- H1.
+    rewrite <- H3.
+    apply s.
+  * discriminate SC2.
+  * inversion SC1. inversion SC2.
+    rewrite <- H2.
+    rewrite <- H4.
+    apply s0.
+Qed.
+
+Lemma cset_open_idempotent : forall i C c,
+  c = open_cc_rec i C c <->
+  (~ (cset_references_bvar i c)) \/ (cset_subset_prop C c /\ cset_references_bvar i C).
+Proof.
+  intros i C c.
+  split.
+  (* -> *)
+  - intros H. destruct (cset_references_bvar_dec i c) eqn:Hic.
+    * csethyp. destruct c ; auto.
+      simpl in Hic.
+      destruct C.
+      ** unfold open_cc_rec in H.
+         rewrite Hic in H.
+         discriminate H.
+      ** inversion H. right. split.
+        *** eapply cset_subset_elem ; csetdec;intros a int1...
+            **** rewrite (NatSetImpl.mem_1 Hic) in H1. inversion H1.
+                 apply (AtomSetImpl.union_2 t int1).
+            **** rewrite (NatSetImpl.mem_1 Hic) in H1.
+                 inversion H1.
+                 apply (NatSetImpl.union_3 (NatSetImpl.remove i t0) int1).
+        *** inversion H. rewrite Hic in H2. rewrite Hic in H1.
+            inversion H2.
+            csetdec.
+            rewrite H4 in Hic.
+            destruct (NatSetImpl.union_1 Hic)...
+            **** destruct ((NatSetImpl.remove_1 (reflexivity i)) H0).
+            **** apply H0.
+    * left. apply cset_not_references_bvar_eq. auto.
+  (* <-  *)
+  - intros H. destruct H.
+    * unfold open_cset.
+      destruct (cset_references_bvar_dec i c) eqn:iINc...
+      rewrite (cset_references_bvar_eq i c) in iINc.
+      contradiction.
+      destruct C; destruct c; simpl...
+      ** reflexivity.
+      ** simpl in H.
+         destruct (NatSetImpl.mem i t0) eqn:iInt0...
+        *** exfalso.
+            apply (H (NatSetImpl.mem_2 iInt0)).
+        *** reflexivity.
+      ** reflexivity.
+      ** simpl in H.
+         destruct (NatSetImpl.mem i t2) eqn:iInt2...
+        *** exfalso.
+            apply (H (NatSetImpl.mem_2 iInt2)).
+        *** reflexivity.
+    * unfold open_cc_rec...
+      destruct C eqn:shpC; destruct c eqn:shpc...
+      ** reflexivity.
+      ** inversion H.
+         simpl in H1.
+         contradiction.
+      ** reflexivity.
+      ** destruct (NatSetImpl.mem i t2) eqn:iInt2...
+        *** f_equal...
+            **** rewrite AtomSetEqual.
+                 intro a. split.
+                 ***** apply AtomSetImpl.union_3.
+                 ***** inversion H.
+                       apply (cset_subset t t0 t1 t2 _ _) in H0.
+                       ****** inversion H0.
+                              intro aIntt1.
+                              apply AtomSetImpl.union_1 in aIntt1.
+                              destruct aIntt1.
+                              ******* apply (H2 a H4).
+                              ******* apply H4.
+                       ****** reflexivity.
+                       ****** reflexivity.
+            **** rewrite NatSetEqual.
+                 intro n. split.
+                  ****** intro nInT2.
+                         destruct (i === n)...
+                         ******* apply NatSetImpl.union_3.
+                                 rewrite <- e.
+                                 inversion H.
+                                 simpl in H1.
+                                 apply H1.
+                         ******* apply NatSetImpl.union_2.
+                                 apply NatSetImpl.remove_2.
+                                 apply n0.
+                                 apply nInT2.
+                  ****** intro nInt2t0.
+                         destruct (i === n).
+                         ******* rewrite e in iInt2.
+                                 apply (NatSetImpl.mem_2 iInt2).
+                         ******* apply NatSetImpl.union_1 in nInt2t0.
+                                 destruct nInt2t0.
+                                 ******** apply (NatSetImpl.remove_3 H0).
+                                 ******** inversion H.
+                                          apply (cset_subset t t0 t1 t2 _ _) in H1.
+                                          inversion H1.
+                                          ********* apply (H4 n H0).
+                                          ********* reflexivity.
+                                          ********* reflexivity.
+        *** reflexivity.
+Qed.
+
+Lemma capture_as_ns_empty : forall C,
+  capture C ->
+  C <> cset_universal ->
+  exists As, C = cset_set As {}N. 
+Proof.
+  intros C H Neq.
+  induction H.
+  * apply (ex_intro _ As).
+    reflexivity.
+  * contradiction.
+Qed.
+
 (** The next lemma is the strengthened induction hypothesis for the
     lemma that follows, which states that opening a locally closed
     term is the identity.  This lemma is not otherwise independently
     useful. *)
 
-Lemma open_tt_rec_type_aux : forall T j V i U,
+Lemma open_ss_rec_shape_aux : forall T j V i U,
   i <> j ->
-  open_tt_rec j V T = open_tt_rec i U (open_tt_rec j V T) ->
-  T = open_tt_rec i U T.
+  open_ss_rec j V T = open_ss_rec i U (open_ss_rec j V T) ->
+  T = open_ss_rec i U T
+with open_st_rec_type_aux : forall T j V i U,
+  i <> j ->
+  open_st_rec j V T = open_st_rec i U (open_st_rec j V T) ->
+  T = open_st_rec i U T.
 Proof with congruence || eauto.
-  induction T; intros j V i U Neq H; simpl in *; inversion H; f_equal...
-  Case "typ_bvar".
-    destruct (j === n)... destruct (i === n)...
+  clear open_ss_rec_shape_aux...
+  ----- intros T j V i U Neq H...
+    induction T...
+    + simpl in *...
+      destruct (i === n)...
+      destruct (j === n)...
+      simpl in *...
+      destruct (i === n)...
+    + simpl in *...
+      f_equal...
+      inversion H...
+      inversion H...
+    + simpl in *...
+      f_equal...
+      apply IHT...
+      inversion H...
+    + simpl in *...
+      f_equal...
+      inversion H...
+  ----- clear open_st_rec_type_aux...
+   intros T j V i U Neq H...
+   induction T...
+   simpl in *...
+   f_equal...
+   inversion H...
 Qed.
 
-(** Opening a locally closed term is the identity.  This lemma depends
-    on the immediately preceding lemma. *)
+Lemma open_ss_open_cs_rec_shape_aux: forall T j C i U,
+  open_cs_rec j C T = open_ss_rec i U (open_cs_rec j C T) ->
+  T = open_ss_rec i U T
+with open_st_open_ct_rec_type_aux: forall T j C i U,
+  open_ct_rec j C T = open_st_rec i U (open_ct_rec j C T) ->
+  T = open_st_rec i U T.
+Proof with congruence || eauto.
+  ----- clear open_ss_open_cs_rec_shape_aux.
+        intros T j C i U H.
+        induction T;simpl in *; inversion H; f_equal...
+  ----- clear open_st_open_ct_rec_type_aux.
+        intros T j C i U H.
+        induction T; simpl in *; inversion H; f_equal...
+Qed.
 
-Lemma open_tt_rec_type : forall T U k,
+Lemma open_cs_open_ss_rec_shape_aux: forall T j V i C,
+  open_ss_rec j V T = open_cs_rec i C (open_ss_rec j V T) ->
+  T = open_cs_rec i C T
+with open_ct_open_st_rec_type_aux: forall T j V i C,
+  open_st_rec j V T = open_ct_rec i C (open_st_rec j V T) ->
+  T = open_ct_rec i C T.
+Proof with congruence || eauto.
+  ----- clear open_cs_open_ss_rec_shape_aux.
+        intros T j V i C H.
+        induction T; simpl in *; inversion H; f_equal...
+  ----- clear open_ct_open_st_rec_type_aux.
+        intros T j V i C H.
+        induction T; simpl in *; inversion H; f_equal...
+Qed.
+
+Lemma open_ss_rec_shape : forall T U k,
+  shape T ->
+  T = open_ss_rec k U T
+with open_st_rec_type : forall T U k,
   type T ->
-  T = open_tt_rec k U T.
+  T = open_st_rec k U T.
 Proof with auto.
-  intros T U k Htyp. revert k.
-  induction Htyp; intros k; simpl; f_equal...
-  Case "typ_all".
-    unfold open_tt in *.
-    pick fresh X.
-    apply (open_tt_rec_type_aux T2 0 (typ_fvar X))...
+  ----- clear open_ss_rec_shape.
+        intros T U k shpT. revert k.
+        induction shpT; intro k; simpl; f_equal; pick fresh X...
+        + unfold open_ct in H0.
+          apply (open_st_open_ct_rec_type_aux _ 0 (cset_fvar X) _ _)...
+        + apply (open_st_rec_type_aux T 0 (shp_fvar X))...
+          apply (open_st_rec_type).
+          apply H.
+          csetdec.
+        + unfold open_ct in H0.
+          apply (open_st_open_ct_rec_type_aux _ 0 (cset_fvar X) _ _)...
+  ----- clear open_st_rec_type.
+        intros T U k shpT. revert k.
+        induction shpT; intro k; simpl; f_equal;pick fresh X...
+Qed.
+
+Lemma open_cc_rec_capture_aux : forall T j V i U,
+  i <> j ->
+  V <> cset_universal ->
+  capture V ->
+  (AtomSetImpl.Empty (AtomSetImpl.inter (fv_cc V) (fv_cc U))) ->
+  open_cc_rec j V T = open_cc_rec i U (open_cc_rec j V T) ->
+  T = open_cc_rec i U T.
+Proof with congruence || eauto.
+  intros T j V i U Neq VFin Closed Disj H.
+  rewrite (cset_open_idempotent i U (open_cc_rec j V T)) in H.
+  rewrite cset_open_idempotent.
+  destruct (cset_references_bvar_dec i T) eqn:Hic.
+  (* i is in c *)
+  - destruct (cset_references_bvar_dec j T) eqn:Hjc ; csethyp...
+    destruct H.
+    * destruct V eqn:shpV; destruct T eqn:shpT; csethyp ; auto.
+      left. simpl in *. rewrite Hjc in H. fnsetdec.
+    * destruct H. destruct U eqn:HC.
+      ** contradiction.
+      ** unfold empty_cset_bvars in Closed. unfold cset_all_bvars in *. destruct V eqn:shpV; destruct T eqn:Hc ; eauto.
+         right. split...
+         inversion H ; csethyp ; simpl in *. constructor. unfold disjoint in *.
+         rewrite Hjc in *. discriminate. rewrite Hjc in *. discriminate. rewrite Hjc in *.
+         constructor...
+         inversion H3.
+         subst.
+         *** intros a aint.
+             destruct (AtomSetImpl.union_1 (H4 a aint)).
+             **** destruct (Disj a (AtomSetImpl.inter_3 H1 aint)).
+             **** apply H1.
+         *** inversion H3.
+             rewrite H8 in H5.
+             destruct (capture_as_ns_empty (cset_set t1 t2) Closed VFin).
+             inversion H6.
+             rewrite H11 in *.
+             intros a aint0...
+             destruct (NatSetImpl.union_1 (H5 a aint0))...
+             **** apply (NatSetImpl.remove_3 H9).
+             **** destruct ((NatSetImpl.empty_1 H9)).
+    * destruct V eqn:shpV; destruct T eqn:shpT; csethyp ; auto.
+      right. simpl in *. rewrite Hjc in H. destruct H...
+      destruct (H (NatSetImpl.mem_2 Hic)). (* fnsetdec. *)
+  (* i is not in c *)
+  - left. apply cset_not_references_bvar_eq. apply Hic.
+Qed.
+
+Lemma open_cc_rec_capture : forall T U k,
+  capture T ->
+  T = open_cc_rec k U T.
+Proof.
+  intros T U k capT.
+  rewrite cset_open_idempotent.
+  left.
+  destruct T.
+  * simpl...
+    unfold not.
+    trivial.
+  * destruct (capture_as_ns_empty (cset_set t t0) capT).
+    ** discriminate.
+    ** inversion H.
+       simpl.
+       apply NatSetImpl.empty_1.
+Qed.
+
+Lemma open_cs_rec_shape_aux : forall T j V i U,
+  i <> j ->
+  V <> cset_universal ->
+  capture V ->
+  (AtomSetImpl.Empty (AtomSetImpl.inter (fv_cc V) (fv_cc U))) ->
+  open_cs_rec j V T = open_cs_rec i U (open_cs_rec j V T) ->
+  T = open_cs_rec i U T
+with open_ct_rec_type_aux : forall T j V i U,
+  i <> j ->
+  V <> cset_universal ->
+  capture V ->
+  (AtomSetImpl.Empty (AtomSetImpl.inter (fv_cc V) (fv_cc U))) ->
+  open_ct_rec j V T = open_ct_rec i U (open_ct_rec j V T) ->
+  T = open_ct_rec i U T.
+Proof with congruence || eauto.
+  clear open_cs_rec_shape_aux.
+  ----- intros T j V i U Neq Vfin capV Disj H.
+        induction T;simpl in *...
+        + f_equal.
+          inversion H...
+          inversion H...
+        + f_equal.
+          inversion H...
+          inversion H...
+        + f_equal.
+          inversion H...
+          apply (open_cc_rec_capture_aux c j V i U)...
+          inversion H...
+  ----- clear open_ct_rec_type_aux.
+        intros T j V i U Neq Vfin capV Disj H.
+        induction T;simpl in *...
+        inversion H.
+        f_equal...
+        apply (open_cc_rec_capture_aux c j V i U)...
+Qed.
+
+Lemma open_cs_rec_shape : forall T U k,
+  shape T ->
+  T = open_cs_rec k U T
+with open_ct_rec_type : forall T U k,
+  type T ->
+  T = open_ct_rec k U T.
+Proof with auto.
+  ----- clear open_cs_rec_shape.
+        intros T U K shpT.
+        induction shpT;simpl in *;f_equal...
+        * pick fresh X.
+          eapply open_ct_rec_type_aux with (V := cset_fvar X) (j := 0);
+            eauto; try solve [discriminate]...
+          constructor...
+          simpl; AtomSetDecide.fsetdec.
+      * pick fresh X.
+          apply (open_ct_open_st_rec_type_aux _ 0 X _ _).
+          apply (open_ct_rec_type (open_st_rec 0 X T) U K).
+          unfold open_st in H.
+          apply (H X)...
+        * apply open_cc_rec_capture...
+        * pick fresh X for (union (union L (union (fv_st T) (fv_ct T))) (fv_cc U)).
+          apply (open_ct_rec_type_aux _ 0 (cset_fvar X) _ _)...
+          discriminate.
+          apply cap_atoms...
+          simpl.
+          intros a aInInter.
+          apply AtomSetFacts.inter_iff in aInInter.
+          destruct aInInter...
+          apply AtomSetImpl.singleton_1 in H1.
+          rewrite H1 in *.
+          auto.
+          apply (open_ct_rec_type (open_ct_rec 0 (cset_fvar X) T) U (S K))...
+          unfold open_ct in H0.
+          apply (H0 X)...
+  ----- clear open_ct_rec_type.
+        intros T U K typT.
+        induction typT...
+        simpl.
+        f_equal...
+        apply open_cc_rec_capture. apply H0.
 Qed.
 
 (** If a name is fresh for a term, then substituting for it is the
     identity. *)
 
-Lemma subst_tt_fresh : forall Z U T,
-   Z `notin` fv_tt T ->
-   T = subst_tt Z U T.
+Lemma subst_ss_fresh : forall Z U T,
+  Z `notin` fv_ss T ->
+  T = subst_ss Z U T
+with subst_st_fresh : forall Z U T,
+  Z `notin` fv_st T ->
+  T = subst_st Z U T.
 Proof with auto.
-  induction T; simpl; intro H; f_equal...
-  Case "typ_fvar".
-    destruct (a == Z)...
-    contradict H; fsetdec.
+  clear subst_ss_fresh.
+  ----- induction T; simpl; intro H; f_equal...
+        + destruct (a === Z)...
+          destruct (H (AtomSetImpl.singleton_2 e)).
+  ----- clear subst_st_fresh.
+        induction T; simpl; intro H; f_equal...   
+Qed.
+ 
+Lemma subst_cs_fresh : forall Z U T,
+  Z `notin` fv_cs T ->
+  T = subst_cs Z U T
+with subst_ct_fresh : forall Z U T,
+  Z `notin` fv_ct T ->
+  T = subst_ct Z U T.
+Proof with auto.
+  clear subst_cs_fresh.
+  ----- induction T; simpl; intro H; f_equal...
+        destruct c.
+        + simpl.
+          reflexivity.
+        + simpl; unfold subst_cc.
+          simpl in H.
+          destruct (AtomSetImpl.mem Z t0) eqn:ZmemT0...
+          exfalso.
+          csetdec.
+  ----- clear subst_ct_fresh.
+        induction T; simpl; intro H; f_equal...
+        destruct c...
+        simpl; unfold subst_cc.
+        simpl in H.
+        destruct (AtomSetImpl.mem Z t) eqn:Zmemt...
+        exfalso.
+        csetdec.
+Qed.
+
+Lemma subst_cc_fresh : forall Z U T,
+  Z `notin` fv_cc T ->
+  T = subst_cc Z U T.
+Proof.
+  induction T; unfold subst_cc; intro H. f_equal...
+  - reflexivity.
+  - destruct (AtomSetImpl.mem Z t) eqn:zInT...
+    * destruct (H (AtomSetImpl.mem_2 zInT)).
+    * reflexivity.
 Qed.
 
 (** Substitution commutes with opening under certain conditions.  This
     lemma depends on the fact that opening a locally closed term is
     the identity. *)
-
-Lemma subst_tt_open_tt_rec : forall T1 T2 X P k,
-  type P ->
-  subst_tt X P (open_tt_rec k T2 T1) =
-    open_tt_rec k (subst_tt X P T2) (subst_tt X P T1).
+Lemma subst_ss_open_ss_rec : forall T1 T2 X P k,
+  shape P ->
+  subst_ss X P (open_ss_rec k T2 T1) = 
+    open_ss_rec k (subst_ss X P T2) (subst_ss X P T1)
+with subst_st_open_st_rec : forall T1 T2 X P k,
+  shape P ->
+  subst_st X P (open_st_rec k T2 T1) = 
+    open_st_rec k (subst_ss X P T2) (subst_st X P T1).
 Proof with auto.
-  intros T1 T2 X P k WP. revert k.
-  induction T1; intros k; simpl; f_equal...
-  Case "typ_bvar".
-    destruct (k === n); subst...
-  Case "typ_fvar".
-    destruct (a == X); subst... apply open_tt_rec_type...
+  ----- clear subst_ss_open_ss_rec.
+        intros T1 T2 X P k WP. revert k.
+        induction T1; intros k; simpl; f_equal...
+        - destruct (k === n); subst...
+        - destruct (a == X); subst... apply open_ss_rec_shape...
+  ----- clear subst_st_open_st_rec.
+        intros T1 T2 X P k WP. revert k.
+        induction T1; intros k; simpl; f_equal...
 Qed.
 
-(** The next lemma is a direct corollary of the immediately preceding
-    lemma---the index is specialized to zero. *)
-
-Lemma subst_tt_open_tt : forall T1 T2 (X:atom) P,
-  type P ->
-  subst_tt X P (open_tt T1 T2) = open_tt (subst_tt X P T1) (subst_tt X P T2).
+Lemma subst_cc_open_cc_rec : forall T1 T2 X P k,
+  capture P ->
+  subst_cc X P (open_cc_rec k T2 T1) = 
+    open_cc_rec k (subst_cc X P T2) (subst_cc X P T1).
 Proof with auto.
-  intros.
-  unfold open_tt.
-  apply subst_tt_open_tt_rec...
+  intros T1 T2 X P k WP. revert k.
+  induction T1; induction T2; induction P; intros k; simpl; unfold subst_cc; f_equal...
+  - destruct (NatSetImpl.mem k t0) eqn:kInt0;destruct (AtomSetImpl.mem X t) eqn:xInt; simpl
+      ;try rewrite kInt0; try rewrite xInt...
+  - destruct (NatSetImpl.mem k t0) eqn:kInt0;destruct (AtomSetImpl.mem X t) eqn:xInt; simpl;
+      try rewrite kInt0; try rewrite xInt...
+    * apply NatSetImpl.mem_2 in kInt0. apply (NatSetImpl.union_2 t2) in kInt0.
+      apply NatSetImpl.mem_1 in kInt0. rewrite kInt0...
+    * destruct (capture_as_ns_empty (cset_set t1 t2) WP)... discriminate.
+      inversion H.
+      rewrite <- union_empty_nats. rewrite kInt0...
+  - destruct (NatSetImpl.mem k t0) eqn:kInt0;destruct (AtomSetImpl.mem X t) eqn:xInt; simpl;
+    try rewrite xInt; try rewrite kInt0...
+    rewrite (AtomSetImpl.mem_1 (AtomSetImpl.union_3 t1 (AtomSetImpl.mem_2 xInt)))...
+    destruct (AtomSetImpl.mem X t1) eqn:xInt1; rewrite mem_union_or_atoms; rewrite xInt1; rewrite xInt...
+  - destruct (capture_as_ns_empty (cset_set t3 t4) WP)... discriminate.
+    inversion H.
+    destruct (NatSetImpl.mem k t0) eqn:kInt0;
+    destruct (AtomSetImpl.mem X t1) eqn:xInt1;
+    destruct (AtomSetImpl.mem X t) eqn: xInt;
+    try rewrite xInt1; try rewrite xInt; simpl; try rewrite xInt; try rewrite kInt0;
+    try rewrite mem_union_or_atoms; try rewrite mem_union_or_nats; 
+    try rewrite xInt1; try rewrite xInt;try rewrite kInt0;simpl;f_equal; repeat try rewrite <- union_empty_nats; try rewrite NatSetFacts.empty_b; try apply AtomSetEqual...
+    * intro a. split; intro aInU; destruct (a == X); apply AtomSetFacts.union_iff in aInU;
+      destruct aInU;csetdec...
+      ** destruct (AtomSetImpl.remove_1 (eq_sym e) H0)...
+      ** apply AtomSetImpl.remove_3 in H0. apply AtomSetFacts.union_iff in H0. destruct H0...
+      ** rewrite e in *. apply AtomSetFacts.union_iff in H0. destruct H0...
+         apply (AtomSetImpl.remove_1 (eq_refl X)) in H0. destruct H0.
+      ** apply AtomSetFacts.union_iff in H0. destruct H0... rewrite e in *.
+         apply (AtomSetImpl.remove_1 (eq_refl X)) in H0. destruct H0.
+      ** apply AtomSetFacts.union_iff in H0. destruct H0... apply AtomSetImpl.remove_3 in H0.
+         apply AtomSetFacts.union_iff. left. apply AtomSetImpl.remove_2...
+      ** apply AtomSetFacts.union_iff in H0. destruct H0...
+         apply AtomSetFacts.union_iff. left.
+         apply AtomSetImpl.remove_3 in H0.
+         apply AtomSetFacts.remove_iff. split...
+    * intro a. split; intro aInU; destruct (a == X); apply AtomSetFacts.union_iff in aInU;
+      destruct aInU...
+      ** destruct (AtomSetImpl.remove_1 (eq_sym e) H0)...
+      ** apply AtomSetImpl.remove_3 in H0. apply AtomSetFacts.union_iff in H0. destruct H0...
+      ** rewrite e in *. apply AtomSetFacts.union_iff in H0. destruct H0...
+         apply (AtomSetImpl.remove_1 (eq_refl X)) in H0. destruct H0.
+      ** apply AtomSetFacts.not_mem_iff in xInt. rewrite e in H0. destruct (xInt H0).
+      ** apply AtomSetFacts.union_iff in H0. destruct H0...
+         apply AtomSetFacts.union_iff. left.
+         apply AtomSetImpl.remove_3 in H0.
+         apply AtomSetFacts.remove_iff. split...
+    * intro a. split; intro aInU; destruct (a == X); apply AtomSetFacts.union_iff in aInU;
+      destruct aInU...
+      ** destruct (AtomSetImpl.remove_1 (eq_sym e) H0)...
+      ** apply AtomSetImpl.remove_3 in H0. apply AtomSetFacts.union_iff in H0. destruct H0...
+      ** csetdec. rewrite e in *. apply AtomSetFacts.not_mem_iff in xInt1...
+      ** apply AtomSetFacts.union_iff in H0. destruct H0... apply AtomSetImpl.remove_1 in H0. destruct H0... apply (eq_sym e).
+      ** apply AtomSetFacts.union_iff in H0. destruct H0...
+         apply AtomSetFacts.union_iff. left.
+         apply AtomSetImpl.remove_3 in H0.
+         apply AtomSetFacts.remove_iff. split...
+Qed.
+
+Lemma subst_cs_open_cs_rec : forall T1 T2 X P k,
+  capture P ->
+  subst_cs X P (open_cs_rec k T2 T1) = 
+    open_cs_rec k (subst_cc X P T2) (subst_cs X P T1)
+with subst_ct_open_ct_rec : forall T1 T2 X P k,
+  capture P ->
+  subst_ct X P (open_ct_rec k T2 T1) = 
+    open_ct_rec k (subst_cc X P T2) (subst_ct X P T1).
+Proof.
+  ----- clear subst_cs_open_cs_rec.
+        intros T1 T2 X P k WP. revert k.
+        induction T1; intros k; simpl; f_equal...
+        - reflexivity.
+        - apply subst_ct_open_ct_rec.
+          apply WP.
+        - apply subst_ct_open_ct_rec.
+          apply WP.
+        - apply IHT1.
+        - apply subst_ct_open_ct_rec.
+          apply WP.
+        - apply subst_cc_open_cc_rec.
+          apply WP.
+        - apply subst_ct_open_ct_rec.
+          apply WP.
+  ----- clear subst_ct_open_ct_rec.
+        intros T1 T2 X P k WP. revert k.
+        induction T1; intros k; simpl; f_equal...
+        apply subst_cs_open_cs_rec; apply WP.
+        apply subst_cc_open_cc_rec; apply WP.
+Qed.
+
+Lemma subst_ss_open_cs_rec : forall Z P k C T,
+  shape P ->
+  subst_ss Z P (open_cs_rec k C T) = open_cs_rec k C (subst_ss Z P T)
+with subst_st_open_ct_rec : forall Z P k C T,
+  shape P ->
+  subst_st Z P (open_ct_rec k C T) = open_ct_rec k C (subst_st Z P T).
+Proof with auto.
+  ----- clear subst_ss_open_cs_rec.
+        intros Z P k C T shpP. revert k.
+        induction T; intro k; simpl; f_equal...
+        destruct (a == Z)...
+        apply open_cs_rec_shape...
+  ----- clear subst_st_open_ct_rec.
+        intros Z P k C T shpP. revert k.
+        induction T; intro k; simpl; f_equal...
+Qed.
+
+Lemma subst_cs_open_ss_rec : forall Z P k C T,
+  subst_cs Z P (open_ss_rec k C T) = open_ss_rec k (subst_cs Z P C) (subst_cs Z P T)
+with subst_ct_open_st_rec : forall Z P k C T,
+  subst_ct Z P (open_st_rec k C T) = open_st_rec k (subst_cs Z P C) (subst_ct Z P T).
+Proof with auto.
+  ----- clear subst_cs_open_ss_rec.
+        intros Z P k C T. revert k.
+        induction T; intro k; simpl; f_equal...
+        destruct (k == n)...
+  ----- clear subst_ct_open_st_rec.
+        intros Z P k C T. revert k.
+        induction T; intro k; simpl; f_equal...
 Qed.
 
 (** The next lemma is a direct corollary of the immediately preceding
@@ -272,16 +947,156 @@ Qed.
     practice, this lemma seems to be needed as a left-to-right rewrite
     rule, when stated in its current form. *)
 
-Lemma subst_tt_open_tt_var : forall (X Y:atom) P T,
+
+Lemma subst_ss_open_ss : forall T1 T2 (X:atom) P,
+  shape P ->
+  subst_ss X P (open_ss T1 T2) = open_ss (subst_ss X P T1) (subst_ss X P T2)
+with subst_st_open_st : forall T1 T2 (X:atom) P,
+  shape P ->
+  subst_st X P (open_st T1 T2) = open_st (subst_st X P T1) (subst_ss X P T2).
+Proof with auto.  
+  ----- clear subst_ss_open_ss.
+        intros T1 T2 X P shpP.
+        apply (subst_ss_open_ss_rec T1 T2 X P 0).
+        apply shpP.
+  ----- clear subst_st_open_st.
+        intros T1 T2 X P shpP.
+        apply (subst_st_open_st_rec T1 T2 X P 0).
+        apply shpP.
+Qed.
+
+Lemma subst_cc_open_cc : forall T1 T2 (X:atom) P,
+  capture P ->
+  subst_cc X P (open_cc T1 T2) = open_cc (subst_cc X P T1) (subst_cc X P T2).
+Proof.
+  intros T1 T2 X P capP.
+  apply (subst_cc_open_cc_rec T1 T2 X P 0).
+  apply capP.
+Qed.
+
+Lemma subst_cs_open_cs : forall T1 T2 (X:atom) P,
+  capture P ->
+  subst_cs X P (open_cs T1 T2) = open_cs (subst_cs X P T1) (subst_cc X P T2)
+with subst_ct_open_ct : forall T1 T2 (X:atom) P,
+  capture P ->
+  subst_ct X P (open_ct T1 T2) = open_ct (subst_ct X P T1) (subst_cc X P T2).
+Proof.
+  ----- clear subst_cs_open_cs.
+        intros T1 T2 X P capP.
+        apply (subst_cs_open_cs_rec T1 T2 X P 0).
+        apply capP.
+  ----- clear subst_ct_open_ct.
+        intros T1 T2 X P capP.
+        apply (subst_ct_open_ct_rec T1 T2 X P 0).
+        apply capP.
+Qed.
+
+Lemma subst_ss_open_cs : forall Z P C T,
+  shape P ->
+  subst_ss Z P (open_cs T C) = open_cs (subst_ss Z P T) C
+with subst_st_open_ct : forall Z P C T,
+  shape P ->
+  subst_st Z P (open_ct T C) = open_ct (subst_st Z P T) C.
+Proof with auto.
+  ----- clear subst_ss_open_cs.
+        intros Z P C T shpP.
+        apply (subst_ss_open_cs_rec _ _ 0 _ _).
+        apply shpP.
+  ----- clear subst_st_open_ct.
+        intros Z P C T shpP.
+        apply (subst_st_open_ct_rec _ _ 0 _ _).
+        apply shpP.
+Qed.
+
+Lemma subst_cs_open_ss : forall Z P C T,
+  subst_cs Z P (open_ss T C) = open_ss (subst_cs Z P T) (subst_cs Z P C)
+with subst_ct_open_st : forall Z P C T,
+  subst_ct Z P (open_st T C) = open_st (subst_ct Z P T) (subst_cs Z P C).
+Proof with auto.
+  ----- clear subst_cs_open_ss.
+        intros Z P C T.
+        apply (subst_cs_open_ss_rec _ _ 0 _ _).
+  ----- clear subst_ct_open_st.
+        intros Z P C T.
+        apply (subst_ct_open_st_rec _ _ 0 _ _).
+Qed.
+
+
+Lemma subst_ss_open_ss_var : forall (X Y:atom) P T,
   Y <> X ->
-  type P ->
-  open_tt (subst_tt X P T) Y = subst_tt X P (open_tt T Y).
+  shape P ->
+  open_ss (subst_ss X P T) Y = subst_ss X P (open_ss T Y)
+with subst_st_open_st_var : forall (X Y:atom) P T,
+  Y <> X ->
+  shape P ->
+  open_st (subst_st X P T) Y = subst_st X P (open_st T Y).
 Proof with congruence || auto.
-  intros X Y P T Neq Wu.
-  unfold open_tt.
-  rewrite subst_tt_open_tt_rec...
-  simpl.
-  destruct (Y == X)...
+  ----- clear subst_ss_open_ss_var.
+        intros X Y P T Neq shpP.
+        rewrite (subst_ss_open_ss T Y X P).
+        f_equal...
+        simpl...
+        destruct (Y === X)...
+        apply shpP.
+  ----- clear subst_st_open_st_var.
+        intros X Y P T Neq shpP.
+        rewrite (subst_st_open_st T Y X P).
+        f_equal...
+        simpl...
+        destruct (Y === X)...
+        apply shpP.
+Qed.
+
+Lemma subst_cc_open_cc_var : forall (X Y:atom) P T,
+  Y <> X ->
+  capture P ->
+  open_cc (subst_cc X P T) (cset_fvar Y) = subst_cc X P (open_cc T (cset_fvar Y)).
+Proof.
+  intros X Y P T Neq capP.
+  rewrite (subst_cc_open_cc T (cset_fvar Y) X P).
+  * rewrite <- (subst_cc_fresh X P (cset_fvar Y)).
+    reflexivity.
+    simpl.
+    solve_notin.
+  * apply capP.
+Qed.
+
+Lemma subst_cs_open_cs_var : forall (X Y:atom) P T,
+  Y <> X ->
+  capture P ->
+  open_cs (subst_cs X P T) (cset_fvar Y) = subst_cs X P (open_cs T (cset_fvar Y))
+with subst_ct_open_ct_var : forall (X Y:atom) P T,
+  Y <> X ->
+  capture P ->
+  open_ct (subst_ct X P T) (cset_fvar Y) = subst_ct X P (open_ct T (cset_fvar Y)).
+Proof.
+  ----- clear subst_cs_open_cs_var.
+        intros X Y P T Neq capP.
+        rewrite (subst_cs_open_cs T (cset_fvar Y) X P).
+        rewrite <- (subst_cc_fresh X P (cset_fvar Y)).
+        * reflexivity.
+        * simpl. solve_notin.
+        * apply capP.
+  ----- clear subst_ct_open_ct_var.
+        intros X Y P T Neq capP.
+        rewrite (subst_ct_open_ct T (cset_fvar Y) X P).
+        rewrite <- (subst_cc_fresh X P (cset_fvar Y)).
+        * reflexivity.
+        * simpl. solve_notin.
+        * apply capP.
+Qed.
+
+Lemma subst_cs_open_ss_var : forall (X : atom) Z P T,
+  subst_cs Z P (open_ss T X) = open_ss (subst_cs Z P T) X
+with subst_ct_open_st_var : forall (X : atom) Z P T,
+  subst_ct Z P (open_st T X) = open_st (subst_ct Z P T) X.
+Proof with auto.
+  ----- clear subst_cs_open_ss_var.
+        intros X Z P T...
+        apply subst_cs_open_ss...
+  ----- clear subst_ct_open_st_var.
+        intros X Z P T.
+        apply subst_ct_open_st...
 Qed.
 
 (** The next lemma states that opening a term is equivalent to first
@@ -289,27 +1104,118 @@ Qed.
     name.  This is actually the strengthened induction hypothesis for
     the version we use in practice. *)
 
-Lemma subst_tt_intro_rec : forall X T2 U k,
-  X `notin` fv_tt T2 ->
-  open_tt_rec k U T2 = subst_tt X U (open_tt_rec k (typ_fvar X) T2).
+Lemma subst_ss_intro_rec : forall X T2 U k,
+  X `notin` fv_ss T2 ->
+  open_ss_rec k U T2 = subst_ss X U (open_ss_rec k (shp_fvar X) T2)
+with subst_st_intro_rec : forall X T2 U k,
+  X `notin` fv_st T2 ->
+  open_st_rec k U T2 = subst_st X U (open_st_rec k (shp_fvar X) T2).
 Proof with congruence || auto.
-  induction T2; intros U k Fr; simpl in *; f_equal...
-  Case "typ_bvar".
-    destruct (k === n)... simpl. destruct (X == X)...
-  Case "typ_fvar".
-    destruct (a == X)... contradict Fr; fsetdec.
+  ----- clear subst_ss_intro_rec.
+        induction T2; intros U k Fr; simpl in *; f_equal...
+        - destruct (k === n)... simpl. destruct (X == X)...
+        - destruct (a == X)... contradict Fr. rewrite e. fsetdec.
+  -----clear subst_st_intro_rec.
+        induction T2; intros U k Fr; simpl in *; f_equal...
 Qed.
+
+Lemma subst_cc_intro_rec : forall X T2 U k,
+  X `notin` fv_cc T2 ->
+  open_cc_rec k U T2 = subst_cc X U (open_cc_rec k (cset_fvar X) T2).
+Proof with congruence || auto.
+  induction T2; intros U k H; unfold subst_cc in *; simpl in *;f_equal...
+  destruct (NatSetImpl.mem k t0) eqn:kInt0...
+  * destruct U; simpl; destruct (AtomSetImpl.mem X (union (singleton X) t)) eqn:xInx... 
+    ** rewrite (AtomSetImpl.mem_1 (AtomSetImpl.union_2 t (AtomSetImpl.singleton_2 (eq_refl X) ))) in xInx.
+       discriminate xInx.
+    ** f_equal...
+       *** rewrite (AtomSetEqual (union t1 t) (union (remove X (union (singleton X) t)) t1)).
+           intro a. split.
+           **** intro aInt1t.
+                apply AtomSetImpl.union_1 in aInt1t.
+                destruct aInt1t.
+                ***** apply AtomSetImpl.union_3.
+                      apply H0.
+                ***** apply AtomSetImpl.union_2.
+                      destruct (a === X) eqn:ax...
+           **** intro aInBig.
+                apply AtomSetImpl.union_1 in aInBig.
+                destruct aInBig.
+                ***** destruct (a === X)...
+                      ****** rewrite e in *.
+                             destruct ((AtomSetImpl.remove_1 (eq_refl X)) H0).
+                      ****** apply AtomSetImpl.union_3.
+                             destruct (AtomSetImpl.union_1 (AtomSetImpl.remove_3 H0)).
+                             ******* destruct (n (eq_sym (AtomSetImpl.singleton_1 H1))).
+                             ******* apply H1.
+                ***** apply AtomSetImpl.union_2.
+                      apply H0.
+       *** apply NatSetEqual.
+           fsetdec.
+    ** rewrite (AtomSetImpl.mem_1 (AtomSetImpl.union_2 t (AtomSetImpl.singleton_2 (eq_refl X) ))) in xInx.
+       discriminate xInx.
+  * simpl.
+    destruct (AtomSetImpl.mem X t) eqn:XInt...
+    exfalso.
+    apply (H (AtomSetImpl.mem_2 XInt)).
+Qed.
+
+Lemma subst_cs_intro_rec : forall X T2 U k,
+  X `notin` fv_cs T2 ->
+  open_cs_rec k U T2 = subst_cs X U (open_cs_rec k (cset_fvar X) T2)
+with subst_ct_intro_rec : forall X T2 U k,
+  X `notin` fv_ct T2 ->
+  open_ct_rec k U T2 = subst_ct X U (open_ct_rec k (cset_fvar X) T2).
+Proof with auto.
+  ----- clear subst_cs_intro_rec.
+        induction T2; intros U k Fr; simpl in *; f_equal...
+        apply subst_cc_intro_rec.
+        destruct c...
+  ----- clear subst_ct_intro_rec.
+        induction T2; intros U k Fr; simpl in *; f_equal...
+        * apply subst_cc_intro_rec. destruct c...
+Qed.
+
 
 (** The next lemma is a direct corollary of the immediately preceding
     lemma---the index is specialized to zero.  *)
 
-Lemma subst_tt_intro : forall X T2 U,
-  X `notin` fv_tt T2 ->
-  open_tt T2 U = subst_tt X U (open_tt T2 X).
+Lemma subst_ss_intro : forall X T2 U,
+  X `notin` fv_ss T2 ->
+  open_ss T2 U = subst_ss X U (open_ss T2 X)
+with subst_st_intro : forall X T2 U,
+  X `notin` fv_st T2 ->
+  open_st T2 U = subst_st X U (open_st T2 X).
+Proof with auto.
+  ----- clear subst_ss_intro.
+        intros.
+        apply subst_ss_intro_rec...
+  ----- clear subst_st_intro.
+        intros.
+        apply subst_st_intro_rec...
+Qed.
+
+Lemma subst_cc_intro : forall X T2 U,
+  X `notin` fv_cc T2 ->
+  open_cc T2 U = subst_cc X U (open_cc T2 (cset_fvar X)).
 Proof with auto.
   intros.
-  unfold open_tt.
-  apply subst_tt_intro_rec...
+  apply subst_cc_intro_rec...
+Qed.
+
+Lemma subst_cs_intro : forall X T2 U,
+  X `notin` fv_cs T2 ->
+  open_cs T2 U = subst_cs X U (open_cs T2 (cset_fvar X))
+with subst_ct_intro : forall X T2 U,
+  X `notin` fv_ct T2 ->
+  open_ct T2 U = subst_ct X U (open_ct T2 (cset_fvar X)).
+Proof with auto.
+  ----- clear subst_cs_intro.
+        intros.
+        apply subst_cs_intro_rec...
+  ----- clear subst_ct_intro.
+        intros.
+        apply subst_ct_intro_rec...
 Qed.
 
 
@@ -321,92 +1227,242 @@ Qed.
     show that substituting a type in a locally-closed expression is
     the identity. *)
 
-Lemma open_te_rec_expr_aux : forall e j u i P ,
-  open_ee_rec j u e = open_te_rec i P (open_ee_rec j u e) ->
-  e = open_te_rec i P e.
+Lemma open_se_rec_expr_aux : forall e j C u i P ,
+  open_ee_rec j u C e = open_se_rec i P (open_ee_rec j u C e) ->
+  e = open_se_rec i P e.
 Proof with congruence || eauto.
-  induction e; intros j u i P H; simpl in *; inversion H; f_equal...
+  induction e; intros j C u i P H; simpl in *; inversion H; f_equal...
 Qed.
 
-Lemma open_te_rec_type_aux : forall e j Q i P,
+Lemma open_ce_rec_expr_aux : forall e j C u i P ,
   i <> j ->
-  open_te_rec j Q e = open_te_rec i P (open_te_rec j Q e) ->
-  e = open_te_rec i P e.
+  C <> cset_universal ->
+  capture C ->
+  AtomSetImpl.Empty (AtomSetImpl.inter (fv_cc C) (fv_cc P)) ->
+  open_ee_rec j u C e = open_ce_rec i P (open_ee_rec j u C e) ->
+  e = open_ce_rec i P e.
+Proof with congruence || eauto.
+  induction e; intros j C u i P Neq UFin capU disj H; simpl in *;inversion H;f_equal...
+  * apply (open_cc_rec_capture_aux c j C i P)...
+Qed.
+
+Lemma open_se_rec_shape_aux : forall e j Q i P,
+  i <> j ->
+  open_se_rec j Q e = open_se_rec i P (open_se_rec j Q e) ->
+  e = open_se_rec i P e.
 Proof.
   induction e; intros j Q i P Neq Heq; simpl in *; inversion Heq;
-    f_equal; eauto using open_tt_rec_type_aux.
+    f_equal; eauto using open_ss_rec_shape_aux; eauto using open_st_rec_type_aux.
 Qed.
 
-Lemma open_te_rec_expr : forall e U k,
+Lemma open_ce_rec_capture_aux : forall e j Q i P,
+  i <> j ->
+  Q <> cset_universal ->
+  capture Q ->
+  AtomSetImpl.Empty (AtomSetImpl.inter (fv_cc Q) (fv_cc P)) ->
+  open_ce_rec j Q e = open_ce_rec i P (open_ce_rec j Q e) ->
+  e = open_ce_rec i P e.
+Proof with auto.
+  induction e; intros j Q i P Neq QFin CapQ Disj Heq; simpl in *; inversion Heq;
+    f_equal; eauto using open_cs_rec_shape_aux; eauto using open_ct_rec_type_aux; eauto using open_cc_rec_capture_aux.
+Qed.
+
+Lemma open_se_open_ce_rec_capture_aux : forall e j C i Sh,
+  open_ce_rec j C e = open_se_rec i Sh (open_ce_rec j C e) ->
+  e = open_se_rec i Sh e.
+Proof with auto.
+  induction e; intros j C i Sh H; simpl in *; inversion H; f_equal;
+  eauto using open_ss_open_cs_rec_shape_aux;
+  eauto using open_st_open_ct_rec_type_aux;
+  eauto using open_cs_open_ss_rec_shape_aux;
+  eauto using open_ct_open_st_rec_type_aux...
+Qed.
+
+Lemma open_ce_open_se_rec_capture_aux : forall e j Sh i C,
+  open_se_rec j Sh e = open_ce_rec i C (open_se_rec j Sh e) ->
+  e = open_ce_rec i C e.
+Proof with auto.
+  induction e; intros j Sh i C H; simpl in *; inversion H; f_equal;
+  eauto using open_ss_open_cs_rec_shape_aux;
+  eauto using open_st_open_ct_rec_type_aux;
+  eauto using open_cs_open_ss_rec_shape_aux;
+  eauto using open_ct_open_st_rec_type_aux;
+  try rewrite <- H2...
+  rewrite <- H1. apply H1.
+Qed.
+
+Lemma open_se_rec_expr : forall e U k,
   expr e ->
-  e = open_te_rec k U e.
-Proof.
+  e = open_se_rec k U e.
+Proof with auto.
   intros e U k WF. revert k.
-  induction WF; intros k; simpl; f_equal; auto using open_tt_rec_type;
-  try solve [
-    unfold open_ee in *;
-    pick fresh x;
-    eapply open_te_rec_expr_aux with (j := 0) (u := exp_fvar x);
-    auto
-  | unfold open_te in *;
-    pick fresh X;
-    eapply open_te_rec_type_aux with (j := 0) (Q := typ_fvar X);
-    auto
-  ].
+  induction WF; intros k; simpl; f_equal; auto using open_ss_rec_shape; auto using open_st_rec_type; unfold open_ee in *.
+  * pick fresh x.
+    apply (open_se_rec_expr_aux e1 0 (cset_fvar x) x _ _ )...
+  * pick fresh x.
+    unfold open_se in *.
+    apply (open_se_rec_shape_aux e1 0 x _ _ )...
+  * pick fresh x.
+    unfold open_ce in *.
+    apply (open_se_open_ce_rec_capture_aux _ 0 (cset_fvar x) _ _)...
 Qed.
 
-Lemma subst_te_fresh : forall X U e,
-  X `notin` fv_te e ->
-  e = subst_te X U e.
+Lemma open_ce_rec_expr : forall e U k,
+  expr e ->
+  e = open_ce_rec k U e.
+Proof with auto.
+  intros e U k WF. revert k.
+  induction WF; intro k; simpl; f_equal...
+  * apply open_ct_rec_type. apply H.
+  * pick fresh X for (union (fv_cc U) L).
+    apply (open_ce_rec_expr_aux _ 0 (cset_fvar X) X _ _)...
+    discriminate.
+    apply cap_atoms...
+    simpl. intros a aInInter.
+    apply AtomSetFacts.inter_iff in aInInter.
+    inversion aInInter.
+    apply AtomSetImpl.singleton_1 in H2.
+    rewrite H2 in Fr.
+    apply (AtomSetImpl.union_2 L) in H3.
+    apply (Fr H3).
+    apply (H1 X)...
+  * apply open_cc_rec_capture...
+  * apply open_cs_rec_shape...
+  * pick fresh X.
+    apply (open_ce_open_se_rec_capture_aux _ 0 X _ _)...
+    unfold open_se in H1.
+    apply (H1 X)...
+  * apply open_cs_rec_shape...
+  * apply open_cc_rec_capture...
+  * pick fresh X for (union (fv_cc U) L).
+    apply (open_ce_rec_capture_aux _ 0 (cset_fvar X) _ _).
+    discriminate. discriminate.
+    apply cap_atoms...
+    simpl. intros a aInInter.
+    apply AtomSetFacts.inter_iff in aInInter.
+    inversion aInInter.
+    apply AtomSetImpl.singleton_1 in H2.
+    rewrite H2 in Fr.
+    apply (AtomSetImpl.union_2 L) in H3.
+    apply (Fr H3).
+    apply (H1 X)...
+  * apply open_cc_rec_capture...
+Qed.
+
+Lemma subst_se_fresh : forall X U e,
+  X `notin` fv_se e ->
+  e = subst_se X U e.
 Proof.
-  induction e; simpl; intros; f_equal; auto using subst_tt_fresh.
+  induction e; simpl; intros; f_equal; auto using subst_ss_fresh; auto using subst_st_fresh.
 Qed.
 
-Lemma subst_te_open_te_rec : forall e T X U k,
-  type U ->
-  subst_te X U (open_te_rec k T e) =
-    open_te_rec k (subst_tt X U T) (subst_te X U e).
+Lemma subst_ce_fresh : forall X U e,
+  X `notin` fv_ce e ->
+  e = subst_ce X U e.
+Proof.
+  induction e; simpl; intros; f_equal; auto using subst_cs_fresh; auto using subst_ct_fresh;
+  auto using subst_cc_fresh.
+Qed.
+
+Lemma subst_se_open_se_rec : forall e T X U k,
+  shape U ->
+  subst_se X U (open_se_rec k T e) =
+    open_se_rec k (subst_ss X U T) (subst_se X U e).
 Proof.
   intros e T X U k WU. revert k.
-  induction e; intros k; simpl; f_equal; auto using subst_tt_open_tt_rec.
+  induction e; intros k; simpl; f_equal; auto using subst_ss_open_ss_rec; auto using subst_st_open_st_rec.
 Qed.
 
-Lemma subst_te_open_te : forall e T X U,
-  type U ->
-  subst_te X U (open_te e T) = open_te (subst_te X U e) (subst_tt X U T).
+Lemma subst_ce_open_ce_rec : forall e T X U k,
+  capture U ->
+  X `notin` fv_cc T ->
+  subst_ce X U (open_ce_rec k T e) =
+    open_ce_rec k (subst_cc X U T) (subst_ce X U e).
+Proof.
+  intros e T X U k WU FninT. revert k.
+  induction e; intros k; simpl; f_equal; auto using subst_cs_open_cs_rec; auto using subst_ct_open_ct_rec; auto using subst_cc_open_cc_rec.
+Qed.
+
+
+Lemma subst_se_open_se : forall e T X U,
+  shape U ->
+  subst_se X U (open_se e T) = open_se (subst_se X U e) (subst_ss X U T).
 Proof with auto.
   intros.
-  unfold open_te.
-  apply subst_te_open_te_rec...
+  unfold open_se.
+  apply subst_se_open_se_rec...
 Qed.
 
-Lemma subst_te_open_te_var : forall (X Y:atom) U e,
+Lemma subst_ce_open_ce : forall e T X U,
+  capture U ->
+  X `notin` fv_cc T ->
+  subst_ce X U (open_ce e T) = open_ce (subst_ce X U e) (subst_cc X U T).
+Proof with auto.
+  intros.
+  unfold open_ce.
+  apply subst_ce_open_ce_rec...
+Qed.
+
+Lemma subst_se_open_se_var : forall (X Y:atom) U e,
   Y <> X ->
-  type U ->
-  open_te (subst_te X U e) Y = subst_te X U (open_te e Y).
+  shape U ->
+  open_se (subst_se X U e) Y = subst_se X U (open_se e Y).
 Proof with congruence || auto.
   intros X Y U e Neq WU.
-  unfold open_te.
-  rewrite subst_te_open_te_rec...
+  unfold open_se.
+  rewrite subst_se_open_se_rec...
   simpl.
   destruct (Y == X)...
 Qed.
 
-Lemma subst_te_intro_rec : forall X e U k,
-  X `notin` fv_te e ->
-  open_te_rec k U e = subst_te X U (open_te_rec k (typ_fvar X) e).
-Proof.
-  induction e; intros U k Fr; simpl in *; f_equal;
-    auto using subst_tt_intro_rec.
+Lemma subst_ce_open_ce_var : forall (X Y:atom) U e,
+  Y <> X ->
+  capture U ->
+  open_ce (subst_ce X U e) (cset_fvar Y) = subst_ce X U (open_ce e (cset_fvar Y)).
+Proof with congruence || auto.
+  intros X Y U e Neq WU.
+  unfold open_ce.
+  rewrite subst_ce_open_ce_rec...
+  repeat (simpl; unfold subst_cc).
+  destruct (AtomSetImpl.mem X (singleton Y)) eqn:xIny...
+  destruct (Neq (AtomSetImpl.singleton_1 (AtomSetImpl.mem_2 xIny))).
 Qed.
 
-Lemma subst_te_intro : forall X e U,
-  X `notin` fv_te e ->
-  open_te e U = subst_te X U (open_te e X).
+Lemma subst_se_intro_rec : forall X e U k,
+  X `notin` fv_se e ->
+  open_se_rec k U e = subst_se X U (open_se_rec k (shp_fvar X) e).
+Proof.
+  induction e; intros U k Fr; simpl in *; f_equal;
+    auto using subst_ss_intro_rec;
+    auto using subst_st_intro_rec.
+Qed.
+
+Lemma subst_ce_intro_rec : forall X e U k,
+  X `notin` fv_ce e ->
+  open_ce_rec k U e = subst_ce X U (open_ce_rec k (cset_fvar X) e).
+Proof.
+  induction e; intros U k Fr; simpl in *; f_equal;
+    auto using subst_cs_intro_rec;
+    auto using subst_ct_intro_rec;
+    auto using subst_cc_intro_rec.
+Qed.
+
+Lemma subst_se_intro : forall X e U,
+  X `notin` fv_se e ->
+  open_se e U = subst_se X U (open_se e X).
 Proof with auto.
   intros.
-  unfold open_te.
-  apply subst_te_intro_rec...
+  unfold open_se.
+  apply subst_se_intro_rec...
+Qed.
+
+Lemma subst_ce_intro : forall X e U,
+  X `notin` fv_ce e ->
+  open_ce e U = subst_ce X U (open_ce e (cset_fvar X)).
+Proof with auto.
+  intros.
+  unfold open_ce.
+  apply subst_ce_intro_rec...
 Qed.
 
 
@@ -415,29 +1471,82 @@ Qed.
 
 (** This section follows the structure of the previous two sections. *)
 
-Lemma open_ee_rec_expr_aux : forall e j v u i,
+Lemma open_ee_rec_expr_aux : forall e j C1 v u C2 i,
   i <> j ->
-  open_ee_rec j v e = open_ee_rec i u (open_ee_rec j v e) ->
-  e = open_ee_rec i u e.
+  C1 <> cset_universal ->
+  capture C1 ->
+  (AtomSetImpl.Empty (AtomSetImpl.inter (fv_cc C1) (fv_cc C2))) ->
+  open_ee_rec j v C1 e = open_ee_rec i u C2 (open_ee_rec j v C1 e) ->
+  e = open_ee_rec i u C2 e.
 Proof with congruence || eauto.
-  induction e; intros j v u i Neq H; simpl in *; inversion H; f_equal...
-  Case "exp_bvar".
-    destruct (j===n)... destruct (i===n)...
+  induction e; intros j C1 v u C2 i Neq C1Fin capC1 Disj H; simpl in *; inversion H; f_equal...
+  destruct (j===n)... destruct (i===n)...
+  apply (open_cc_rec_capture_aux c j C1 i C2)...
 Qed.
 
-Lemma open_ee_rec_type_aux : forall e j V u i,
-  open_te_rec j V e = open_ee_rec i u (open_te_rec j V e) ->
-  e = open_ee_rec i u e.
+Lemma open_ee_rec_shape_aux : forall e j C V u i,
+  open_se_rec j V e = open_ee_rec i u C (open_se_rec j V e) ->
+  e = open_ee_rec i u C e.
 Proof.
-  induction e; intros j V u i H; simpl; inversion H; f_equal; eauto.
+  induction e; intros j C V u i H; simpl; inversion H; f_equal; eauto.
+  rewrite <- H2.
+  apply H2.
 Qed.
 
-Lemma open_ee_rec_expr : forall u e k,
+Lemma open_ee_rec_capture_aux : forall e j C V u i,
+  i <> j ->
+  V <> cset_universal ->
+  capture V ->
+  AtomSetImpl.Empty (AtomSetImpl.inter (fv_cc V) (fv_cc C)) ->
+  open_ce_rec j V e = open_ee_rec i u C (open_ce_rec j V e) ->
+  e = open_ee_rec i u C e.
+Proof.
+  induction e; intros j C V u i Neq Vfin CapV Disj H; simpl; inversion H; f_equal; eauto.
+  apply open_cc_rec_capture_aux in H2.
+  apply H2. apply Neq. apply Vfin. apply CapV. apply Disj.
+Qed.
+
+
+Lemma open_ee_rec_expr : forall e u C k,
   expr e ->
-  e = open_ee_rec k u e.
+  e = open_ee_rec k u C e.
 Proof with auto.
-  intros u e k Hexpr. revert k.
-  induction Hexpr; intro k; simpl; f_equal; auto*;
+  intros e u C k WF; revert k; induction WF; intro k; simpl; f_equal...
+  * pick fresh x for (union L (fv_cc C)).
+    apply (open_ee_rec_expr_aux _ 0 (cset_fvar x) x _ _ _).
+    discriminate. discriminate. apply cap_atoms...
+    intros a aInInter. apply AtomSetFacts.inter_iff in aInInter. simpl in *. inversion aInInter.
+    apply AtomSetImpl.singleton_1 in H2.
+    rewrite H2 in *.
+    apply (AtomSetImpl.union_3 L) in H3.
+    apply (Fr H3)...
+    unfold open_ee in H1.
+    apply (H1 x)...
+  * apply open_cc_rec_capture...
+  * pick fresh x for (union L (fv_cc C)).
+    apply (open_ee_rec_shape_aux _ 0 C x _ _).
+    unfold open_se in H1.
+    apply (H1 x)...
+  * pick fresh x for (union L (fv_cc C)).
+    apply (open_ee_rec_capture_aux _ 0 _ (cset_fvar x) _ _)...
+    discriminate. apply cap_atoms...
+    intros a aInInter. apply AtomSetFacts.inter_iff in aInInter. simpl in *. inversion aInInter.
+    apply AtomSetImpl.singleton_1 in H2.
+    rewrite H2 in *.
+    apply (AtomSetImpl.union_3 L) in H3.
+    apply (Fr H3)...
+    unfold open_ce in H1.
+    apply (H1 x)...
+Qed.
+(*
+  intros u e C k Hexpr Cfin. revert k.
+  induction Hexpr; intro k; simpl; f_equal...
+  * pick fresh x.
+    apply (open_ee_rec_expr_aux e1 0 C0 x _ _ _)...
+    unfold open_ee in *.
+    CFin
+    destruct (capture_as_ns_empty C0 H0).
+    csetdec.
   try solve [
     unfold open_ee in *;
     pick fresh x;
@@ -448,117 +1557,227 @@ Proof with auto.
     eapply open_ee_rec_type_aux with (j := 0) (V := typ_fvar X);
     auto
   ].
+ *)
+
+Lemma subst_ee_fresh : forall (x: atom) U u e,
+  x `notin` (fv_ee e `union` fv_ce e) ->
+  e = subst_ee x U u e.
+Proof with auto using subst_cc_fresh, subst_ct_fresh, subst_cs_fresh.
+  intros *; induction e; simpl; intro H; f_equal...
+  - destruct (a==x)...
+    exfalso. AtomSetDecide.fsetdec.
 Qed.
 
-Lemma subst_ee_fresh : forall (x: atom) u e,
-  x `notin` fv_ee e ->
-  e = subst_ee x u e.
-Proof with auto.
-  intros x u e; induction e; simpl; intro H; f_equal...
-  Case "exp_fvar".
-    destruct (a==x)...
-    contradict H; fsetdec.
-Qed.
-
-Lemma subst_ee_open_ee_rec : forall e1 e2 x u k,
+Lemma subst_ee_open_ee_rec : forall e1 C e2 x U u k,
   expr u ->
-  subst_ee x u (open_ee_rec k e2 e1) =
-    open_ee_rec k (subst_ee x u e2) (subst_ee x u e1).
+  capture U ->
+  C <> cset_universal ->
+  subst_ee x U u (open_ee_rec k e2 C e1) =
+    open_ee_rec k (subst_ee x U u e2) (subst_cc x U C) (subst_ee x U u e1).
 Proof with auto.
-  intros e1 e2 x u k WP. revert k.
+  intros * WP WU CFin. revert k.
   induction e1; intros k; simpl; f_equal...
   Case "exp_bvar".
     destruct (k === n); subst...
   Case "exp_fvar".
     destruct (a == x); subst... apply open_ee_rec_expr...
+  Case "exp_capp".
+    rewrite <- subst_cc_open_cc_rec...
 Qed.
 
-Lemma subst_ee_open_ee : forall e1 e2 x u,
+Lemma subst_ee_open_ee : forall e1 e2 C x U u,
+  capture U ->
   expr u ->
-  subst_ee x u (open_ee e1 e2) =
-    open_ee (subst_ee x u e1) (subst_ee x u e2).
+  C <> cset_universal ->
+  subst_ee x U u (open_ee e1 e2 C) =
+    open_ee (subst_ee x U u e1) (subst_ee x U u e2) (subst_cc x U C).
 Proof with auto.
   intros.
   unfold open_ee.
   apply subst_ee_open_ee_rec...
 Qed.
 
-Lemma subst_ee_open_ee_var : forall (x y:atom) u e,
+Lemma subst_ee_open_ee_var : forall (x y:atom) u U e C,
   y <> x ->
+  capture U ->
   expr u ->
-  open_ee (subst_ee x u e) y = subst_ee x u (open_ee e y).
+  C <> cset_universal ->
+  open_ee (subst_ee x U u e) y (subst_cc x U C) = subst_ee x U u (open_ee e y C).
 Proof with congruence || auto.
-  intros x y u e Neq Wu.
+  intros * Neq WU Wu CFin.
   unfold open_ee.
   rewrite subst_ee_open_ee_rec...
   simpl.
   destruct (y == x)...
 Qed.
 
-Lemma subst_te_open_ee_rec : forall e1 e2 Z P k,
-  subst_te Z P (open_ee_rec k e2 e1) =
-    open_ee_rec k (subst_te Z P e2) (subst_te Z P e1).
+Lemma subst_se_open_ce_rec : forall Z P e k C,
+  shape P ->
+  subst_se Z P (open_ce_rec k C e) = open_ce_rec k C (subst_se Z P e).
 Proof with auto.
-  induction e1; intros e2 Z P k; simpl; f_equal...
+  intros Z P e k C shpP. revert k.
+  induction e; intro k; simpl; f_equal...
+  * apply subst_st_open_ct_rec...
+  * apply subst_ss_open_cs_rec...
+  * apply subst_ss_open_cs_rec...
+Qed.
+
+Lemma subst_se_open_ee_rec : forall e1 C e2 Z P k,
+  subst_se Z P (open_ee_rec k e2 C e1) =
+    open_ee_rec k (subst_se Z P e2) C (subst_se Z P e1).
+Proof with auto.
+  induction e1; intros C e2 Z P k; simpl; f_equal...
   Case "exp_bvar".
     destruct (k === n)...
 Qed.
 
-Lemma subst_te_open_ee : forall e1 e2 Z P,
-  subst_te Z P (open_ee e1 e2) = open_ee (subst_te Z P e1) (subst_te Z P e2).
+Lemma subst_ce_open_se_rec : forall e1 Z  Q P k,
+  capture P ->
+  subst_ce Z P (open_se_rec k Q e1) =
+    open_se_rec k (subst_cs Z P Q) (subst_ce Z P e1).
+Proof with auto.
+  induction e1; intros Z Q P k capP; simpl; f_equal...
+  apply subst_ct_open_st_rec...
+  apply subst_cs_open_ss_rec...
+  apply subst_cs_open_ss_rec...
+Qed.
+
+
+Lemma subst_ce_open_se: forall Z P Q e,
+  capture P ->
+  subst_ce Z P (open_se e Q) =
+    open_se  (subst_ce Z P e) (subst_cs Z P Q).
+Proof with auto.
+  intros Z P e C shpP.
+  apply (subst_ce_open_se_rec _ _ _ _ _ )...
+Qed.
+
+Lemma subst_ce_open_ee_rec : forall e1 C e2 Z P k,
+  capture P ->
+  subst_ce Z P (open_ee_rec k e2 C e1) =
+    open_ee_rec k (subst_ce Z P e2) (subst_cc Z P C) (subst_ce Z P e1).
+Proof with auto.
+  induction e1; intros C e2 Z P k capP; simpl; f_equal...
+  Case "exp_bvar".
+    destruct (k === n)...
+  apply subst_cc_open_cc_rec...
+Qed.
+
+Lemma subst_se_open_ce: forall Z P e C,
+  shape P ->
+  subst_se Z P (open_ce e C) = open_ce (subst_se Z P e) C.
+Proof with auto.
+  intros Z P e C shpP.
+  apply (subst_se_open_ce_rec _ _ _ 0 _ )...
+Qed.
+
+Lemma subst_se_open_ee : forall e1 C e2 Z P,
+  subst_se Z P (open_ee e1 e2 C) = open_ee (subst_se Z P e1)(subst_se Z P e2) C.
 Proof with auto.
   intros.
   unfold open_ee.
-  apply subst_te_open_ee_rec...
+  apply subst_se_open_ee_rec...
 Qed.
 
-Lemma subst_te_open_ee_var : forall Z (x:atom) P e,
-  open_ee (subst_te Z P e) x = subst_te Z P (open_ee e x).
+Lemma subst_ce_open_ee : forall e1 C e2 Z P,
+  capture P ->
+  subst_ce Z P (open_ee e1 e2 C) = open_ee (subst_ce Z P e1)(subst_ce Z P e2) (subst_cc Z P C).
 Proof with auto.
   intros.
-  rewrite subst_te_open_ee...
+  unfold open_ee.
+  apply subst_ce_open_ee_rec...
 Qed.
 
-Lemma subst_ee_open_te_rec : forall e P z u k,
-  expr u ->
-  subst_ee z u (open_te_rec k P e) = open_te_rec k P (subst_ee z u e).
+Lemma subst_se_open_ee_var : forall Z (x:atom) P e C,
+  open_ee (subst_se Z P e) x C = subst_se Z P (open_ee e x C).
 Proof with auto.
-  induction e; intros P z u k H; simpl; f_equal...
+  intros.
+  rewrite subst_se_open_ee...
+Qed.
+
+Lemma subst_ce_open_ee_var : forall Z (x:atom) P e C,
+  capture P ->
+  open_ee (subst_ce Z P e) x (subst_cc Z P C) = subst_ce Z P (open_ee e x C).
+Proof with auto.
+  intros.
+  rewrite subst_ce_open_ee...
+Qed.
+
+Lemma subst_ee_open_se_rec : forall e P z U u k,
+  capture U ->
+  expr u ->
+  subst_ee z U u (open_se_rec k P e) = open_se_rec k (subst_cs z U P) (subst_ee z U u e).
+Proof with auto using subst_ct_open_st_rec, subst_cs_open_ss_rec.
+  induction e; intros * WU Wu; simpl; f_equal...
   Case "exp_fvar".
-    destruct (a == z)... apply open_te_rec_expr...
+    destruct (a == z)... apply open_se_rec_expr...
 Qed.
 
-Lemma subst_ee_open_te : forall e P z u,
+Lemma subst_ee_open_ce_rec : forall e P z U u k,
+  capture U ->
   expr u ->
-  subst_ee z u (open_te e P) = open_te (subst_ee z u e) P.
+  subst_ee z U u (open_ce_rec k P e) = open_ce_rec k (subst_cc z U P) (subst_ee z U u e).
+Proof with auto using subst_ct_open_ct_rec, subst_cc_open_cc_rec, subst_cs_open_cs_rec.
+  induction e; intros * WU Wu; simpl; f_equal...
+  Case "exp_fvar".
+    destruct (a == z)... apply open_ce_rec_expr...
+Qed.
+
+Lemma subst_ee_open_se : forall e P z U u,
+  capture U ->
+  expr u ->
+  subst_ee z U u (open_se e P) = open_se (subst_ee z U u e) (subst_cs z U P).
+Proof with auto using subst_ct_open_ct_rec, subst_cc_open_cc_rec, subst_cs_open_cs_rec.
+  intros.
+  unfold open_se.
+  apply subst_ee_open_se_rec...
+Qed.
+
+Lemma subst_ee_open_ce : forall e P z U u,
+  capture U ->
+  expr u ->
+  subst_ee z U u (open_ce e P) = open_ce (subst_ee z U u e) (subst_cc z U P).
 Proof with auto.
   intros.
-  unfold open_te.
-  apply subst_ee_open_te_rec...
+  unfold open_ce.
+  apply subst_ee_open_ce_rec...
 Qed.
 
-Lemma subst_ee_open_te_var : forall z (X:atom) u e,
+Lemma subst_ee_open_se_var : forall z (X:atom) u U e,
+  capture U ->
   expr u ->
-  open_te (subst_ee z u e) X = subst_ee z u (open_te e X).
+  open_se (subst_ee z U u e) X = subst_ee z U u (open_se e X).
 Proof with auto.
-  intros z X u e H.
-  rewrite subst_ee_open_te...
+  intros * WU Wu.
+  rewrite subst_ee_open_se...
 Qed.
 
-Lemma subst_ee_intro_rec : forall x e u k,
-  x `notin` fv_ee e ->
-  open_ee_rec k u e = subst_ee x u (open_ee_rec k (exp_fvar x) e).
-Proof with congruence || auto.
-  induction e; intros u k Fr; simpl in *; f_equal...
+Lemma subst_ee_open_ce_var : forall z (X:atom) U u e,
+  z <> X ->
+  capture U ->
+  expr u ->
+  open_ce (subst_ee z U u e) (cset_fvar X) = subst_ee z U u (open_ce e (cset_fvar X)).
+Proof with auto.
+  intros * Fr WU Wu.
+  rewrite subst_ee_open_ce...
+    repeat(simpl; unfold subst_cc); destruct (AtomSetImpl.mem z (singleton X)) eqn:HX...
+    exfalso. rewrite <- AtomSetFacts.mem_iff in *. AtomSetDecide.fsetdec.
+Qed.
+
+Lemma subst_ee_intro_rec : forall x e u k C,
+  x `notin` (fv_ee e) `union` (fv_ce e)->
+  open_ee_rec k u C e = (subst_ee x C u (open_ee_rec k (exp_fvar x) (cset_fvar x) e)).
+Proof with congruence || auto using subst_cc_intro_rec, subst_ct_fresh, subst_cs_fresh, subst_cc_fresh.
+  induction e; intros * Fr; simpl in *; f_equal...
   Case "exp_bvar".
     destruct (k === n)... simpl. destruct (x == x)...
   Case "exp_fvar".
-    destruct (a == x)... contradict Fr; fsetdec.
+    destruct (a == x)... AtomSetDecide.fsetdec.
 Qed.
 
-Lemma subst_ee_intro : forall x e u,
-  x `notin` fv_ee e ->
-  open_ee e u = subst_ee x u (open_ee e x).
+Lemma subst_ee_intro : forall x e u C,
+  x `notin` fv_ee e `union` (fv_ce e) ->
+  open_ee e u C = subst_ee x C u (open_ee e x (cset_fvar x)).
 Proof with auto.
   intros.
   unfold open_ee.
@@ -574,128 +1793,153 @@ Qed.
 
 (** The following lemma depends on [subst_tt_open_tt_var]. *)
 
-Lemma subst_tt_type : forall Z P T,
+Lemma subst_cc_capture : forall Z C D,
+  capture C ->
+  capture D ->
+  capture (subst_cc Z C D).
+Proof with eauto.
+  intros Z C D capC capD.
+  induction C; induction D...
+  * unfold subst_cc...
+    destruct (AtomSetImpl.mem Z t)...
+  * unfold subst_cc...
+    destruct (AtomSetImpl.mem Z t1)...
+    apply capture_as_ns_empty in capC...
+    apply capture_as_ns_empty in capD...
+    destruct capC; destruct capD...
+    inversion H. inversion H0...
+    rewrite <- (union_empty_nats {}N).
+    apply cap_atoms...
+    discriminate. discriminate.
+Qed.
+
+Lemma subst_ss_shape : forall Z P T,
+  shape T ->
+  shape P ->
+  shape (subst_ss Z P T)
+with subst_st_type : forall Z P T,
   type T ->
-  type P ->
-  type (subst_tt Z P T).
+  shape P ->
+  type (subst_st Z P T).
 Proof with auto.
-  intros Z P T HT HP.
-  induction HT; simpl...
-  Case "type_fvar".
-    destruct (X == Z)...
-  Case "type_all".
-    pick fresh Y and apply type_all...
-    rewrite subst_tt_open_tt_var...
+  ----- clear subst_ss_shape. intros Z P T HT HP.
+        induction HT; simpl...
+        * destruct (X == Z)...
+        * pick fresh Y and apply shape_arrow...
+          rewrite <- subst_st_open_ct...
+        * pick fresh Y and apply shape_sall...
+          rewrite subst_st_open_st_var...
+        * pick fresh Y and apply shape_call...
+          rewrite <- subst_st_open_ct...
+  ----- clear subst_st_type. intros Z P T HT HP.
+        induction HT; simpl...
+Qed.
+
+Lemma subst_cs_shape : forall Z P T,
+  shape T ->
+  capture P ->
+  shape (subst_cs Z P T)
+with subst_ct_type : forall Z P T,
+  type T ->
+  capture P ->
+  type (subst_ct Z P T).
+Proof with auto using subst_cc_capture.
+  ----- clear subst_cs_shape. intros Z P T HT HP.
+        induction HT; simpl...
+        * pick fresh Y and apply shape_arrow...
+          rewrite subst_ct_open_ct_var...
+        * pick fresh Y and apply shape_sall...
+          rewrite <- subst_ct_open_st_var...
+        * pick fresh Y and apply shape_call...
+          rewrite subst_ct_open_ct_var...
+  ----- clear subst_ct_type. intros Z P T HT HP.
+        induction HT; simpl...
 Qed.
 
 (** The following lemma depends on [subst_tt_type],
     [subst_te_open_ee_var], and [sbust_te_open_te_var]. *)
 
-Lemma subst_te_expr : forall Z P e,
+Lemma subst_se_expr : forall Z P e,
   expr e ->
-  type P ->
-  expr (subst_te Z P e).
-Proof with eauto using subst_tt_type.
+  shape P ->
+  expr (subst_se Z P e).
+Proof with eauto using subst_ss_shape.
   intros Z P e He Hp.
-  induction He; simpl; auto using subst_tt_type;
-  try solve [
-    econstructor;
-    try instantiate (1 := L `union` singleton Z);
-    intros;
-    try rewrite subst_te_open_ee_var;
-    try rewrite subst_te_open_te_var;
-    instantiate;
-    eauto using subst_tt_type
-  ].
+  induction He; simpl; auto using subst_ss_shape; auto using subst_st_type.
+  * apply (expr_abs L (subst_st Z P T) (subst_se Z P e1)).
+    apply subst_st_type...
+    intros x xnInl.
+    rewrite subst_se_open_ee_var...
+  * apply (expr_sabs (AtomSetImpl.union L (AtomSetImpl.singleton Z)) (subst_ss Z P Sh) (subst_se Z P e1)).
+    apply subst_ss_shape...
+    intros.
+    rewrite subst_se_open_se_var...
+  * apply (expr_cabs L C (subst_se Z P e1)).
+    apply H.
+    intros.
+    rewrite <- subst_se_open_ce.
+    apply (H1 X)...
+    apply Hp.
+Qed.
+
+Lemma subst_ce_expr : forall Z P e,
+  expr e ->
+  capture P ->
+  expr (subst_ce Z P e).
+Proof with eauto.
+  intros Z P e exprE capP.
+  induction exprE; simpl; auto using subst_cs_shape; auto using subst_ct_type; auto using subst_cc_capture...
+  * apply expr_abs with (L:=(union L {{ Z }}))...
+    ** apply subst_ct_type...
+    ** intros x xnInL.
+       replace (exp_fvar x) with (subst_ce Z P x) by auto...
+       replace (cset_fvar x) with (subst_cc Z P (cset_fvar x))...
+       rewrite <- subst_ce_open_ee...
+       unfold subst_cc; simpl...
+       replace (AtomSetImpl.mem Z (singleton x)) with false...
+       symmetry.
+       apply AtomSetFacts.not_mem_iff...
+  * apply expr_sabs with (L:=(union L {{ Z }}))...
+    ** apply subst_cs_shape...
+    ** intros x xnInL.
+       replace (shp_fvar x) with (subst_cs Z P x) by auto...
+       rewrite <- subst_ce_open_se...
+  * apply expr_cabs with (L:=(union L {{ Z }}))...
+    ** apply subst_cc_capture...
+    ** intros X XnInL.
+       replace (cset_fvar X) with (subst_cc Z P (cset_fvar X)).
+       rewrite <- subst_ce_open_ce...
+       unfold subst_cc; simpl...
+       replace (AtomSetImpl.mem Z (singleton X)) with false...
+       symmetry.
+       apply AtomSetFacts.not_mem_iff...
 Qed.
 
 (** The following lemma depends on [subst_ee_open_ee_var] and
     [subst_ee_open_te_var]. *)
 
-Lemma subst_ee_expr : forall z e1 e2,
+Lemma subst_ee_expr : forall z e1 C e2,
+  capture C ->
   expr e1 ->
   expr e2 ->
-  expr (subst_ee z e2 e1).
-Proof with auto.
-  intros z e1 e2 He1 He2.
-  induction He1; simpl; auto;
-  try solve [
-    econstructor;
-    try instantiate (1 := L `union` singleton z);
-    intros;
-    try rewrite subst_ee_open_ee_var;
-    try rewrite subst_ee_open_te_var;
-    instantiate;
-    auto
-  ].
-  Case "expr_var".
-    destruct (x == z)...
-Qed.
-
-
-(* *********************************************************************** *)
-(** * #<a name="body"></a># Properties of [body_e] *)
-
-(** The two kinds of facts we need about [body_e] are the following:
-      - How to use it to derive that terms are locally closed.
-      - How to derive it from the facts that terms are locally closed.
-
-    Since we use it only in the context of [exp_let] and [exp_sum]
-    (see the definition of reduction), those two constructors are the
-    only ones we consider below. *)
-
-Lemma expr_let_from_body : forall e1 e2,
-  expr e1 ->
-  body_e e2 ->
-  expr (exp_let e1 e2).
-Proof.
-  intros e1 e2 H [J1 J2].
-  pick fresh y and apply expr_let; auto.
-Qed.
-
-Lemma body_from_expr_let : forall e1 e2,
-  expr (exp_let e1 e2) ->
-  body_e e2.
-Proof.
-  intros e1 e2 H.
-  unfold body_e.
-  inversion H; eauto.
-Qed.
-
-Lemma expr_case_from_body : forall e1 e2 e3,
-  expr e1 ->
-  body_e e2 ->
-  body_e e3 ->
-  expr (exp_case e1 e2 e3).
-Proof.
-  intros e1 e2 e3 H [J1 J2] [K1 K2].
-  pick fresh y and apply expr_case; auto.
-Qed.
-
-Lemma body_inl_from_expr_case : forall e1 e2 e3,
-  expr (exp_case e1 e2 e3) ->
-  body_e e2.
-Proof.
-  intros e1 e2 e3 H.
-  unfold body_e.
-  inversion H; eauto.
-Qed.
-
-Lemma body_inr_from_expr_case : forall e1 e2 e3,
-  expr (exp_case e1 e2 e3) ->
-  body_e e3.
-Proof.
-  intros e1 e2 e3 H.
-  unfold body_e.
-  inversion H; eauto.
-Qed.
-
-Lemma open_ee_body_e : forall e1 e2,
-  body_e e1 -> expr e2 -> expr (open_ee e1 e2).
-Proof.
-  intros e1 e2 [L H] J.
-  pick fresh x.
-  rewrite (subst_ee_intro x); auto using subst_ee_expr.
+  expr (subst_ee z C e2 e1).
+Proof with eauto using subst_cc_capture, subst_ct_type, subst_cs_shape.
+  intros * HC He1 He2.
+  induction He1; simpl; unfold subst_cc; auto...
+  * destruct (x == z)...
+  * eapply expr_abs with (L := L `union` (singleton z))...
+    intros. replace (cset_fvar x) with (subst_cc z C (cset_fvar x))...
+    rewrite subst_ee_open_ee_var; simpl...
+    discriminate.
+    repeat (simpl; unfold subst_cc). 
+    destruct (AtomSetImpl.mem z (singleton x)) eqn:HZ...
+    rewrite <- AtomSetFacts.mem_iff in *. AtomSetDecide.fsetdec...
+  * eapply expr_sabs with (L := L `union` (singleton z))...
+    intros.
+    rewrite subst_ee_open_se_var...
+  * eapply expr_cabs with (L := L `union` (singleton z))...
+    intros...
+    rewrite subst_ee_open_ce_var...
 Qed.
 
 
@@ -706,19 +1950,24 @@ Qed.
     substitution.  This is part of our strategy for automatically
     discharging local-closure proof obligations. *)
 
-#[export] Hint Resolve subst_tt_type subst_te_expr subst_ee_expr : core.
+#[export] Hint Resolve 
+  subst_ss_shape subst_st_type  subst_ct_type subst_se_expr subst_ee_expr subst_ce_expr
+  subst_cc_capture : core.
 
 (** We also add as hints the lemmas concerning [body_e]. *)
-
-#[export] Hint Resolve expr_let_from_body body_from_expr_let : core.
-#[export] Hint Resolve expr_case_from_body : core.
-#[export] Hint Resolve body_inl_from_expr_case body_inr_from_expr_case : core.
-#[export] Hint Resolve open_ee_body_e : core.
 
 (** When reasoning about the [binds] relation and [map], we
     occasionally encounter situations where the binding is
     over-simplified.  The following hint undoes that simplification,
     thus enabling [Hint]s from the MetatheoryEnv library. *)
 
-#[export] Hint Extern 1 (binds _ (?F (subst_tt ?X ?U ?T)) _) =>
-  unsimpl (subst_tb X U (F T)) : core.
+#[export] Hint Extern 1 (binds _ (?F (subst_ss ?X ?U ?T)) _) =>
+  unsimpl (subst_sb X U (F T)) : core.
+#[export] Hint Extern 1 (binds _ (?F (subst_st ?X ?U ?T)) _) =>
+  unsimpl (subst_sb X U (F T)) : core.
+#[export] Hint Extern 1 (binds _ (?F (subst_cc ?X ?U ?T)) _) =>
+  unsimpl (subst_cb X U (F T)) : core.
+#[export] Hint Extern 1 (binds _ (?F (subst_cs ?X ?U ?T)) _) =>
+  unsimpl (subst_cb X U (F T)) : core.
+#[export] Hint Extern 1 (binds _ (?F (subst_ct ?X ?U ?T)) _) =>
+  unsimpl (subst_cb X U (F T)) : core.
