Fsub/Fsub_LetSum_Lemmas.v
@@ -30,28 +30,127 @@ Require Export Fsub.Fsub_LetSum_Infrastructure.
 (** If a type is well-formed in an environment, then it is locally
     closed. *)
 
-Lemma type_from_wf_typ : forall E T,
-  wf_typ E T -> type T.
+Lemma union_rewrite : forall S1 S2 (t : atom),
+  t `notin` (union S1 S2) <->
+  (t `notin` S1) /\ (t `notin` S2).
+Proof.
+  intros S1 S2 t.
+  split; intro H.
+  * split; auto.
+  * intro nIn. inversion H.
+    apply AtomSetFacts.union_iff in nIn.
+    destruct nIn; auto.
+Qed.
+
+Lemma capture_from_wf_cap : forall E C,
+  wf_cap E C -> capture C.
 Proof.
   intros E T H; induction H; eauto.
+Qed.
+
+Lemma shape_from_wf_shp : forall E Sh,
+  wf_shp E Sh -> shape Sh
+with type_from_wf_typ : forall E T,
+  wf_typ E T -> type T.
+Proof.
+  ----- clear shape_from_wf_shp.
+        intros E T H; induction H; eauto.
+        * eapply shape_call...
+          apply (capture_from_wf_cap E C H).
+          intros.
+          apply (type_from_wf_typ (X ~ bind_sub_cap C ++ E) (open_ct T (cset_fvar X)) (H0 X H1)).
+  ----- clear type_from_wf_typ.
+        intros E T H; induction H.
+        apply (type_pair S C (shape_from_wf_shp E S H) (capture_from_wf_cap E C H0)).
 Qed.
 
 (** The remaining properties are analogous to the properties that we
     need to show for the subtyping and typing relations. *)
 
-Lemma wf_typ_weakening : forall T E F G,
+Lemma wf_cap_weakening : forall C E F G,
+  wf_cap (G ++ E) C ->
+  uniq (G ++ F ++ E) ->
+  wf_cap (G ++ F ++ E) C.
+Proof with simpl_env; eauto.
+  intros C E F G Hwf_cap Hk.
+  remember (G ++ E) as F'.
+  generalize dependent G.
+  induction Hwf_cap; intros G Hok Heq; subst...
+  apply wf_cset_set...
+  intros a aNinA.
+  rewrite <- app_assoc.
+  destruct (H a)...
+  * left. destruct H0.
+    eapply ex_intro.
+    apply binds_app_iff in H0. destruct H0...
+  * right. destruct H0.
+    eapply ex_intro.
+    apply binds_app_iff in H0. destruct H0...
+Qed.
+
+Lemma wf_shp_weakening : forall Sh E F G,
+  wf_shp (G ++ E) Sh ->
+  uniq (G ++ F ++ E) ->
+  wf_shp (G ++ F ++ E) Sh
+with wf_typ_weakening : forall T E F G,
   wf_typ (G ++ E) T ->
   uniq (G ++ F ++ E) ->
   wf_typ (G ++ F ++ E) T.
 Proof with simpl_env; eauto.
-  intros T E F G Hwf_typ Hk.
-  remember (G ++ E) as F'.
-  generalize dependent G.
-  induction Hwf_typ; intros G Hok Heq; subst...
-  Case "type_all".
-    pick fresh Y and apply wf_typ_all...
-    rewrite <- app_assoc.
-    apply H0...
+  ----- clear wf_shp_weakening.
+        intros Sh E F G Hwf_shp Hk.
+        remember (G ++ E) as F'.
+        generalize dependent G.
+        induction Hwf_shp; intros G Hok Heq; subst...
+        * apply (wf_shp_arrow (union L (union (dom E) (union (dom F) (dom G)))) _ _)...
+          intros X XnInL.
+          apply (wf_typ_weakening _ E F (X ~ bind_typ T1 ++ G)).
+          apply (H0 X)...
+          apply uniq_cons...
+        * apply (wf_shp_sall (union L (union (dom E) (union (dom F) (dom G)))) _ _)...
+          intros X XnInL.
+          eapply (wf_typ_weakening (open_st T X) E F (X ~ bind_sub_shp S ++ G) _)...
+          Unshelve.
+          rewrite app_assoc.
+          eapply (H X _).
+          Unshelve.
+          solve_notin.
+        * apply (wf_shp_call (union L (union (dom E) (union (dom F) (dom G)))) _ _)...
+          ** apply wf_cap_weakening...
+          ** intros X XnInL.
+             eapply (wf_typ_weakening (open_ct T (cset_fvar X)) E F (X ~ bind_sub_cap C ++ G) _)...
+             Unshelve.
+             rewrite app_assoc.
+              eapply (H0 X _).
+              Unshelve.
+              solve_notin.
+  ----- clear wf_typ_weakening.
+        intros Sh E F G Hwf_typ Hk.
+        remember (G ++ E) as F'.
+        generalize dependent G.
+        induction Hwf_typ; intros G Hok Heq; subst...
+        apply wf_pair...
+        apply wf_cap_weakening...
+Qed.
+
+Lemma wf_cap_weaken_head : forall C E F,
+  wf_cap E C ->
+  uniq (F ++ E) ->
+  wf_cap (F ++ E) C.
+Proof.
+  intros.
+  rewrite_env (empty ++ F ++ E).
+  auto using wf_cap_weakening.
+Qed.
+
+Lemma wf_shp_weaken_head : forall Sh E F,
+  wf_shp E Sh ->
+  uniq (F ++ E) ->
+  wf_shp (F ++ E) Sh.
+Proof.
+  intros.
+  rewrite_env (empty ++ F++ E).
+  auto using wf_shp_weakening.
 Qed.
 
 Lemma wf_typ_weaken_head : forall T E F,
@@ -64,73 +163,825 @@ Proof.
   auto using wf_typ_weakening.
 Qed.
 
-Lemma wf_typ_narrowing : forall V U T E F X,
-  wf_typ (F ++ X ~ bind_sub V ++ E) T ->
-  wf_typ (F ++ X ~ bind_sub U ++ E) T.
+Lemma wf_cap_narrowing_shp : forall V U C E F X,
+  wf_cap (F ++ X ~ bind_sub_shp V ++ E) C ->
+  wf_cap (F ++ X ~ bind_sub_shp U ++ E) C.
 Proof with simpl_env; eauto.
-  intros V U T E F X Hwf_typ.
-  remember (F ++ X ~ bind_sub V ++ E) as G.
+  intros V U T E F X Hwf_cap.
+  remember (F ++ X ~ bind_sub_shp V ++ E) as G.
   generalize dependent F.
-  induction Hwf_typ; intros F Heq; subst...
-  Case "wf_typ_var".
-    analyze_binds H...
-  Case "typ_all".
-    pick fresh Y and apply wf_typ_all...
-    rewrite <- app_assoc.
-    apply H0...
+  induction Hwf_cap; intros F Heq; subst...
+  apply wf_cset_set...
+  intros a anInA.
+  destruct (H a)...
+  * left. destruct H0.
+    eapply ex_intro.
+    apply binds_app_1 in H0.
+    destruct H0.
+    ** apply binds_app_2. apply H0.
+    ** apply binds_app_1 in H0.
+       destruct H0.
+       *** apply binds_one_iff in H0.
+           inversion H0.
+           discriminate H2.
+       *** apply binds_app_3. apply binds_app_3. apply H0.
+  * right. destruct H0. 
+    eapply ex_intro.
+    apply binds_app_1 in H0.
+    destruct H0.
+    ** apply binds_app_2. apply H0.
+    ** apply binds_app_1 in H0.
+       destruct H0.
+       *** apply binds_one_iff in H0.
+           inversion H0.
+           discriminate H2.
+       *** apply binds_app_3. apply binds_app_3. apply H0.
 Qed.
 
-Lemma wf_typ_strengthening : forall E F x U T,
- wf_typ (F ++ x ~ bind_typ U ++ E) T ->
- wf_typ (F ++ E) T.
+Lemma wf_cap_narrowing_cap : forall V U C E F X,
+  wf_cap (F ++ X ~ bind_sub_cap V ++ E) C ->
+  wf_cap (F ++ X ~ bind_sub_cap U ++ E) C.
+Proof with simpl_env; eauto.
+  intros V U T E F X Hwf_cap.
+  remember (F ++ X ~ bind_sub_cap V ++ E) as G.
+  generalize dependent F.
+  induction Hwf_cap; intros F Heq; subst...
+  apply wf_cset_set...
+  intros a anInA.
+  destruct (H a anInA).
+  * left. destruct (X == a);destruct H0...
+    apply binds_app_1 in H0.
+    destruct H0.
+    ** eapply ex_intro. apply binds_app_iff. left.
+       apply H0.
+    ** apply binds_app_1 in H0. destruct H0.
+       *** eapply ex_intro. apply binds_app_iff. right. apply binds_app_iff. left.
+           apply binds_one...
+           apply binds_one_iff in H0.
+           inversion H0...
+       *** eapply ex_intro. apply binds_app_iff. right. apply binds_app_iff. right.
+           apply H0.
+  * right. destruct (X == a);destruct H0...
+    apply binds_app_1 in H0.
+    destruct H0.
+    ** eapply ex_intro.
+       apply binds_app_2. apply H0.
+    ** apply binds_app_1 in H0.
+       destruct H0.
+       *** eapply ex_intro.
+           apply binds_one_iff in H0.
+           inversion H0.
+           discriminate H2.
+           Unshelve.
+           apply (pair shp_top (cset_set {} {}N)).
+       *** eapply ex_intro.
+           apply binds_app_3. apply binds_app_3. apply H0.
+    ** eapply ex_intro.
+       apply binds_app_iff in H0.
+       destruct H0...
+       apply binds_app_iff in H0.
+       destruct H0...
+       apply binds_one_iff in H0.
+       inversion H0...
+       symmetry in H1. destruct (n H1).
+Qed.
+
+Lemma wf_cap_narrowing_typ : forall V U C E F X,
+  wf_cap (F ++ X ~ bind_typ V ++ E) C ->
+  wf_cap (F ++ X ~ bind_typ U ++ E) C.
+Proof with simpl_env; eauto.
+  intros V U T E F X Hwf_cap.
+  remember (F ++ X ~ bind_typ V ++ E) as G.
+  generalize dependent F.
+  induction Hwf_cap; intros F Heq; subst...
+  apply wf_cset_set...
+  intros a anInA.
+  destruct (H a)...
+  * left. destruct H0.
+    eapply ex_intro.
+    apply binds_app_1 in H0.
+    destruct H0.
+    ** apply binds_app_2. apply H0.
+    ** apply binds_app_1 in H0.
+       destruct H0.
+       *** apply binds_one_iff in H0.
+           inversion H0.
+           discriminate H2.
+       *** apply binds_app_3. apply binds_app_3. apply H0.
+  * right. destruct H0 as [T BindsA]. 
+    analyze_binds BindsA...
+Qed.
+
+Lemma wf_shp_narrowing_shp : forall V U Sh E F X,
+  wf_shp (F ++ X ~ bind_sub_shp V ++ E) Sh ->
+  wf_shp (F ++ X ~ bind_sub_shp U ++ E) Sh
+with wf_typ_narrowing_shp :  forall V U T E F X,
+  wf_typ (F ++ X ~ bind_sub_shp V ++ E) T ->
+  wf_typ (F ++ X ~ bind_sub_shp U ++ E) T.
+Proof with simpl_env; eauto.
+  ----- clear wf_shp_narrowing_shp.
+        intros V U T E F X Hwf_shp.
+        remember (F ++ X ~ bind_sub_shp V ++ E) as G.
+        generalize dependent F.
+        induction Hwf_shp; intros F Heq; subst...
+        * destruct (x == X)...
+        * apply (wf_shp_arrow L _ _ _)...
+          intros x xnInL.
+          apply (wf_typ_narrowing_shp V _ _ _ (x ~ bind_typ T1 ++ F) _).
+          apply (H0 x xnInL).
+        * apply (wf_shp_sall L (F ++ X ~ bind_sub_shp U ++ E) S T).
+          ** apply (IHHwf_shp F)...
+          ** intros X0 X0nInL.
+             apply (wf_typ_narrowing_shp V U (open_st T X0) E (X0 ~ bind_sub_shp S ++ F) X)...
+        * apply (wf_shp_call L (F ++ X ~ bind_sub_shp U ++ E) C T).
+          ** apply (wf_cap_narrowing_shp V _ _ _ _ _)...
+          ** intros X0 X0nInL.
+              apply (wf_typ_narrowing_shp V U (open_ct T (cset_fvar X0)) E (X0 ~ bind_sub_cap C ++ F) X)...
+  ----- clear wf_typ_narrowing_shp.
+        intros V U T E F X Hwf_shp.
+        remember (F ++ X ~ bind_sub_shp V ++ E) as G.
+        generalize dependent F.
+        induction Hwf_shp; intros F Heq; subst...
+        apply wf_pair.
+        * apply (wf_shp_narrowing_shp V _ _ _ _ _)...
+        * apply (wf_cap_narrowing_shp V _ _ _ _ _)...
+Qed.
+
+Lemma wf_shp_narrowing_cap : forall V U Sh E F X,
+  wf_shp (F ++ X ~ bind_sub_cap V ++ E) Sh ->
+  wf_shp (F ++ X ~ bind_sub_cap U ++ E) Sh
+with wf_typ_narrowing_cap :  forall V U T E F X,
+  wf_typ (F ++ X ~ bind_sub_cap V ++ E) T ->
+  wf_typ (F ++ X ~ bind_sub_cap U ++ E) T.
+Proof with simpl_env; eauto.
+  ----- clear wf_shp_narrowing_cap.
+        intros V U T E F X Hwf_shp.
+        remember (F ++ X ~ bind_sub_cap V ++ E) as G.
+        generalize dependent F.
+        induction Hwf_shp; intros F Heq; subst...
+        * destruct (x == X)... rewrite e in H.
+          apply binds_app_1 in H.
+          destruct H.
+          ** apply (wf_shp_fvar _ U0).
+             apply binds_app_2. rewrite e. apply H.
+          ** apply binds_app_1 in H. destruct H.
+             *** apply binds_one_iff in H.
+                 inversion H.
+                 discriminate H1.
+             *** apply (wf_shp_fvar _ U0).
+                 apply binds_app_3. apply binds_app_3.
+                 rewrite e. apply H.
+        * apply (wf_shp_arrow L _ _ _)...
+          intros X0 X0nInL.
+          apply (wf_typ_narrowing_cap V _ _ _ (X0 ~ bind_typ T1 ++ F) _).
+          apply (H0 X0 X0nInL).
+        * apply (wf_shp_sall L (F ++ X ~ bind_sub_cap U ++ E) S T).
+          ** apply (IHHwf_shp F)...
+          ** intros X0 X0nInL.
+             apply (wf_typ_narrowing_cap V U (open_st T X0) E (X0 ~ bind_sub_shp S ++ F) X)...
+        * apply (wf_shp_call L (F ++ X ~ bind_sub_cap U ++ E) C T).
+          ** apply (wf_cap_narrowing_cap V _ _ _ _ _)...
+          ** intros X0 X0nInL.
+              apply (wf_typ_narrowing_cap V U (open_ct T (cset_fvar X0)) E (X0 ~ bind_sub_cap C ++ F) X)...
+  ----- clear wf_typ_narrowing_cap.
+        intros V U T E F X Hwf_shp.
+        remember (F ++ X ~ bind_sub_cap V ++ E) as G.
+        generalize dependent F.
+        induction Hwf_shp; intros F Heq; subst...
+        apply wf_pair.
+        * apply (wf_shp_narrowing_cap V _ _ _ _ _)...
+        * apply (wf_cap_narrowing_cap V _ _ _ _ _)...
+Qed.
+
+Lemma wf_shp_narrowing_typ : forall V U Sh E F X,
+  wf_shp (F ++ X ~ bind_typ V ++ E) Sh ->
+  wf_shp (F ++ X ~ bind_typ U ++ E) Sh
+with wf_typ_narrowing_typ :  forall V U T E F X,
+  wf_typ (F ++ X ~ bind_typ V ++ E) T ->
+  wf_typ (F ++ X ~ bind_typ U ++ E) T.
+Proof with simpl_env; eauto.
+  ----- clear wf_shp_narrowing_typ.
+        intros V U T E F X Hwf_shp.
+        remember (F ++ X ~ bind_typ V ++ E) as G.
+        generalize dependent F.
+        induction Hwf_shp; intros F Heq; subst...
+        * destruct (x == X); subst...
+          analyze_binds H...  
+        * apply (wf_shp_arrow L _ _ _)...
+          intros x xnInL.
+          apply (wf_typ_narrowing_typ V _ _ _ (x ~ bind_typ T1 ++ F) _).
+          apply (H0 x xnInL).
+        * apply (wf_shp_sall L (F ++ X ~ bind_typ U ++ E) S T).
+          ** apply (IHHwf_shp F)...
+          ** intros X0 X0nInL.
+             apply (wf_typ_narrowing_typ V U (open_st T X0) E (X0 ~ bind_sub_shp S ++ F) X)...
+        * apply (wf_shp_call L (F ++ X ~ bind_typ U ++ E) C T).
+          ** apply (wf_cap_narrowing_typ V _ _ _ _ _)...
+          ** intros X0 X0nInL.
+             eapply (wf_typ_narrowing_typ V U (open_ct T (cset_fvar X0)) E (X0 ~ bind_sub_cap C ++ F) X)...
+  ----- clear wf_typ_narrowing_typ.
+        intros V U T E F X Hwf_shp.
+        remember (F ++ X ~ bind_typ V ++ E) as G.
+        generalize dependent F.
+        induction Hwf_shp; intros F Heq; subst...
+        apply wf_pair.
+        * apply (wf_shp_narrowing_typ V _ _ _ _ _)...
+        * apply (wf_cap_narrowing_typ V _ _ _ _ _)...
+Qed.
+
+
+Lemma wf_cap_strengthening_shp : forall E F x U T,
+ wf_cap (F ++ x ~ bind_sub_shp U ++ E) T ->
+ wf_cap (F ++ E) T.
 Proof with simpl_env; eauto.
   intros E F x U T H.
-  remember (F ++ x ~ bind_typ U ++ E) as G.
+  remember (F ++ x ~ bind_sub_shp U ++ E) as G.
   generalize dependent F.
   induction H; intros F Heq; subst...
-  Case "wf_typ_var".
-    analyze_binds H...
-  Case "wf_typ_all".
-    pick fresh Y and apply wf_typ_all...
-    rewrite <- app_assoc.
-    apply H1...
+  apply wf_cset_set...
+  intros a aInA.
+  destruct (H a aInA).
+  * left. destruct (x == a); destruct H0...
+    ** apply binds_app_iff in H0.
+       destruct H0.
+       *** eapply ex_intro.
+           apply binds_app_2.
+           apply H0.
+       *** apply binds_app_iff in H0. destruct H0.
+           **** eapply ex_intro.
+                apply binds_one_iff in H0.
+                inversion H0.
+                discriminate H2.
+                Unshelve.
+                apply x0.
+           **** eapply ex_intro.
+                apply binds_app_3.
+                apply H0.
+    ** apply binds_app_iff in H0.
+       destruct H0.
+       *** eapply ex_intro.
+           apply binds_app_2.
+           apply H0.
+        *** apply binds_app_iff in H0. destruct H0.
+           **** eapply ex_intro.
+                apply binds_one_iff in H0.
+                inversion H0.
+                symmetry in H1.
+                destruct (n H1).
+                Unshelve.
+                apply x0.
+           **** eapply ex_intro.
+                apply binds_app_3.
+                apply H0.
+  * right. destruct (x == a); destruct H0...
+    ** apply binds_app_iff in H0.
+       destruct H0.
+       *** eapply ex_intro.
+           apply binds_app_2.
+           apply H0.
+       *** apply binds_app_iff in H0. destruct H0.
+           **** eapply ex_intro.
+                apply binds_one_iff in H0.
+                inversion H0.
+                discriminate H2.
+                Unshelve.
+                apply x0.
+           **** eapply ex_intro.
+                apply binds_app_3.
+                apply H0.
+    ** apply binds_app_iff in H0.
+       destruct H0.
+       *** eapply ex_intro.
+           apply binds_app_2.
+           apply H0.
+        *** apply binds_app_iff in H0. destruct H0.
+           **** eapply ex_intro.
+                apply binds_one_iff in H0.
+                inversion H0.
+                discriminate H2.
+                Unshelve.
+                apply x0.
+           **** eapply ex_intro.
+                apply binds_app_3.
+                apply H0.
 Qed.
 
-Lemma wf_typ_subst_tb : forall F Q E Z P T,
-  wf_typ (F ++ Z ~ bind_sub Q ++ E) T ->
-  wf_typ E P ->
-  uniq (map (subst_tb Z P) F ++ E) ->
-  wf_typ (map (subst_tb Z P) F ++ E) (subst_tt Z P T).
+Lemma subst_sb_cap_iden : forall U Z P,
+  subst_sb Z P (bind_sub_cap U) = bind_sub_cap U.
+Proof.
+  intros U Z P.
+  auto.
+Qed.
+
+Lemma subst_cb_cap : forall U Z P,
+  subst_cb Z P (bind_sub_cap U) = bind_sub_cap (subst_cc Z P U).
+Proof.
+  intros U Z P.
+  auto.
+Qed.
+
+Lemma subst_sb_typ : forall V Z P,
+  subst_sb Z P (bind_typ V) = bind_typ (subst_st Z P V).
+Proof.
+  intros V Z P.
+  auto.
+Qed.
+
+Lemma subst_sb_shp : forall V Z P,
+  subst_sb Z P (bind_sub_shp V) = bind_sub_shp (subst_ss Z P V).
+Proof.
+  intros V Z P.
+  auto.
+Qed.
+
+Lemma subst_ss_atom : forall Sh A X,
+  X <> A ->
+  (subst_ss A Sh X) = X.
+Proof.
+  intros Sh A X XNA.
+  simpl.
+  destruct (X == A).
+  * destruct (XNA e).
+  * reflexivity.
+Qed.
+
+Lemma wf_cap_subst_sbs : forall F Q E Z P T,
+  wf_cap (F ++ Z ~ bind_sub_shp Q ++ E) T ->
+  wf_shp E P ->
+  uniq (map (subst_sb Z P) F ++ E) ->
+  wf_cap (map (subst_sb Z P) F ++ E) T.
 Proof with simpl_env; eauto using wf_typ_weaken_head, type_from_wf_typ.
   intros F Q E Z P T WT WP.
-  remember (F ++ Z ~ bind_sub Q ++ E) as G.
+  remember (F ++ Z ~ bind_sub_shp Q ++ E) as G.
   generalize dependent F.
-  induction WT; intros F EQ Ok; subst; simpl subst_tt...
-  Case "wf_typ_var".
-    destruct (X == Z); subst...
-    SCase "X <> Z".
-      analyze_binds H...
-      apply (wf_typ_var (subst_tt Z P U))...
-  Case "wf_typ_all".
-    pick fresh Y and apply wf_typ_all...
-    rewrite subst_tt_open_tt_var...
-    rewrite_env (map (subst_tb Z P) (Y ~ bind_sub T1 ++ F) ++ E).
-    apply H0...
+  induction WT; intros F EQ Ok; subst...
+  apply wf_cset_set.
+  intros a aIna.
+  destruct (H a aIna).
+  * left. destruct H0. apply binds_app_iff in H0.
+    destruct H0...
+    ** eapply ex_intro. apply binds_app_iff.
+       left.
+       rewrite <- (subst_sb_cap_iden _ Z P).
+       apply (binds_map_2 _ _ (subst_sb Z P) _ ).
+       apply H0.
+    ** apply binds_app_iff in H0. destruct H0.
+       *** eapply ex_intro. apply binds_one_iff in H0.
+           inversion H0. discriminate H2.
+           Unshelve. apply x.
+       *** eapply ex_intro. apply binds_app_iff. right. apply H0.
+  * right. destruct H0. apply binds_app_iff in H0.
+    destruct H0...
+    ** eapply ex_intro. apply binds_app_iff.
+       left.
+       Unshelve.
+       2 : {
+        apply (subst_st Z P x).
+       }
+       rewrite <- subst_sb_typ.
+       apply binds_map_2.
+       apply H0.
+    ** apply binds_app_iff in H0. destruct H0.
+       *** eapply ex_intro. apply binds_one_iff in H0.
+           inversion H0. discriminate H2. Unshelve. apply x.
+       *** eapply ex_intro. apply binds_app_iff. right. apply H0.
 Qed.
 
-Lemma wf_typ_open : forall E U T1 T2,
+Lemma wf_shp_subst_sbs : forall F Q E Z P T,
+  wf_shp (F ++ Z ~ bind_sub_shp Q ++ E) T ->
+  wf_shp E P ->
+  uniq (map (subst_sb Z P) F ++ E) ->
+  wf_shp (map (subst_sb Z P) F ++ E) (subst_ss Z P T)
+with wf_typ_subst_sbs : forall F Q E Z P T,
+  wf_typ (F ++ Z ~ bind_sub_shp Q ++ E) T ->
+  wf_shp E P ->
+  uniq (map (subst_sb Z P) F ++ E) ->
+  wf_typ (map (subst_sb Z P) F ++ E) (subst_st Z P T).
+Proof with simpl_env; eauto using
+  wf_typ_weaken_head, type_from_wf_typ, shape_from_wf_shp.
+----- 
+  clear wf_shp_subst_sbs.
+  intros F Q E Z P T WT WP.
+  remember (F ++ Z ~ bind_sub_shp Q ++ E) as G.
+  generalize dependent F.
+  induction WT; intros F EQ Ok; subst; simpl subst_ss...
+  * destruct (x == Z)...
+    ** apply wf_shp_weaken_head...
+    ** apply binds_app_iff in H. destruct H.
+        *** apply (wf_shp_fvar _ (subst_ss Z P U) _).
+            apply binds_app_iff.
+            left.
+            rewrite <- subst_sb_shp.
+            apply binds_map_2.
+            apply H.
+        *** apply binds_app_iff in H. destruct H.
+            **** apply binds_one_iff in H. inversion H.
+                destruct (n H0).
+            **** apply (wf_shp_fvar _ U _).
+                apply binds_app_iff. right. apply H.
+  * apply (wf_shp_arrow (union (union L (union (dom F) (dom E))) {{ Z }}) _ _)...
+    intros X XnInL.
+    rewrite <- subst_st_open_ct...
+    rewrite_env ((map (subst_sb Z P) (X ~ bind_typ T1 ++ F) ++ E)).
+    apply (wf_typ_subst_sbs _ Q _ _ _ _)...
+  * apply (wf_shp_sall (union (union L (union (dom F) (dom E))) {{ Z }}) _ _)...
+    ** intros X XninL. rewrite <- subst_sb_shp. rewrite <- app_assoc.
+        rewrite <- map_cons. rewrite <- (subst_ss_atom P Z X)...
+        rewrite <- subst_st_open_st.
+        rewrite <- app_assoc.
+        rewrite <- map_cons.
+        apply (wf_typ_subst_sbs _ Q _ _ _ _)...
+        apply (shape_from_wf_shp E P)...
+  * apply (wf_shp_call (union (union L (union (dom F) (dom E))) {{ Z }}) _ _)...
+    ** apply (wf_cap_subst_sbs _ Q _ _ _ _)...
+    ** intros X XnInL.
+        rewrite <- (subst_sb_cap_iden _ Z P)...
+        rewrite <- app_assoc.
+        rewrite <- map_cons.
+        unfold open_ct.
+        erewrite  <- subst_st_open_ct_rec.
+        eapply wf_typ_subst_sbs...
+        eapply shape_from_wf_shp...
+-----
+  clear wf_typ_subst_sbs.
+  intros F Q E Z P T WT WP.
+  remember (F ++ Z ~ bind_sub_shp Q ++ E) as G.
+  generalize dependent F.
+  induction WT; intros F EQ Ok; subst; simpl subst_ss...
+  apply wf_pair.
+  * induction P...
+  * apply (wf_cap_subst_sbs _ Q _ _ _ _)...
+Qed.
+
+Lemma union_empty:
+  (NatSetImpl.union {}N {}N) = {}N.
+Proof.
+  apply NatSetEqual.
+  split; intros H.
+  * apply NatSetImpl.union_1 in H. destruct H; auto.
+  * apply NatSetImpl.empty_1 in H. destruct H.
+Qed.
+#[export] Hint Rewrite union_empty : core.
+
+Lemma wf_cap_subst_cbc : forall F Q E Z P T,
+  wf_cap (F ++ Z ~ bind_sub_cap Q ++ E) T ->
+  wf_cap E P ->
+  uniq (map (subst_cb Z P) F ++ E) ->
+  wf_cap (map (subst_cb Z P) F ++ E) (subst_cc Z P T).
+Proof with simpl_env; eauto using wf_cap_weaken_head, capture_from_wf_cap.
+  intros F Q E Z P T WT WP.
+  remember (F ++ Z ~ bind_sub_cap Q ++ E) as G.
+  generalize dependent F.
+  induction WT; intros F EQ Ok; subst...
+  repeat (simpl; unfold subst_cc).
+  destruct (AtomSetImpl.mem Z A) eqn:ZinA... destruct P...
+  * destruct (capture_as_ns_empty (cset_set t t0))... discriminate.
+    inversion H0; subst...
+    rewrite union_empty.
+    apply (wf_cset_set (map (subst_cb Z (cset_set x {}N)) F ++ E) (union (remove Z A) x)).
+    intros a aIna.
+    (* I am not entirely sure about how to procede here, if a `in` A, we can apply H
+       but if a `in` x, I am not certain.
+       
+       If a `in` x, note that x is well formed in E*)
+    inversion WP; subst...
+    rewrite AtomSetFacts.union_iff in aIna; destruct aIna as [InRemove | InX]...
+    + assert (a `in` A). AtomSetDecide.fsetdec.
+      assert (a <> Z). AtomSetDecide.fsetdec.
+      destruct (H a) as [[U BindsU] | [V BindsV]]...
+      - analyze_binds BindsU...
+        left; eexists.
+        apply binds_app_2...
+        eapply binds_map_2 with (f := subst_cb Z (cset_set x {}N)) in BindsTac...
+      - analyze_binds BindsV...
+        right; eexists.
+        apply binds_app_2...
+        eapply binds_map_2 with (f := subst_cb Z (cset_set x {}N)) in BindsTac...
+    + destruct (H3 a) as [[U BindsU] | [V BindsV]]...
+  *  apply (wf_cset_set (map (subst_cb Z P) F ++ E) A).
+    intros a aInA.
+    destruct (H a aInA)...
+    ** left. destruct H0. apply binds_app_1 in H0. destruct H0.
+       *** eexists.
+           apply binds_app_2.
+           eapply binds_map_2 with (f := subst_cb Z P) in H0...
+       *** analyze_binds H0...
+           exfalso. rewrite <- AtomSetFacts.not_mem_iff in ZinA...
+             (* For Ed, nothing bad, just didn't get a chance to finish this off *)
+    ** right. destruct H0. apply binds_app_1 in H0. destruct H0.
+      *** eexists.
+          apply binds_app_2.
+          eapply binds_map_2 with (f := subst_cb Z P) in H0...
+      *** analyze_binds H0...
+Qed.
+
+Lemma wf_cap_subst_cbt : forall F Q E Z P T,
+  wf_cap (F ++ Z ~ bind_typ Q ++ E) T ->
+  wf_cap E P ->
+  uniq (map (subst_cb Z P) F ++ E) ->
+  wf_cap (map (subst_cb Z P) F ++ E) (subst_cc Z P T).
+Proof with simpl_env; eauto using wf_cap_weaken_head, capture_from_wf_cap.
+  intros F Q E Z P T WT WP.
+  remember (F ++ Z ~ bind_typ Q ++ E) as G.
+  generalize dependent F.
+  induction WT; intros F EQ Ok; subst...
+  repeat (simpl; unfold subst_cc).
+  destruct (AtomSetImpl.mem Z A) eqn:ZinA... destruct P...
+  * destruct (capture_as_ns_empty (cset_set t t0))... discriminate.
+    inversion H0; subst...
+    rewrite union_empty.
+    apply (wf_cset_set (map (subst_cb Z (cset_set x {}N)) F ++ E) (union (remove Z A) x)).
+    intros a aIna.
+    (* I am not entirely sure about how to procede here, if a `in` A, we can apply H
+       but if a `in` x, I am not certain.
+       
+       If a `in` x, note that x is well formed in E*)
+    inversion WP; subst...
+    rewrite AtomSetFacts.union_iff in aIna; destruct aIna as [InRemove | InX]...
+    + assert (a `in` A). AtomSetDecide.fsetdec.
+      assert (a <> Z). AtomSetDecide.fsetdec.
+      destruct (H a) as [[U BindsU] | [V BindsV]]...
+      - analyze_binds BindsU...
+        left; eexists.
+        apply binds_app_2...
+        eapply binds_map_2 with (f := subst_cb Z (cset_set x {}N)) in BindsTac...
+      - analyze_binds BindsV...
+        right; eexists.
+        apply binds_app_2...
+        eapply binds_map_2 with (f := subst_cb Z (cset_set x {}N)) in BindsTac...
+    + destruct (H3 a) as [[U BindsU] | [V BindsV]]...
+  *  apply (wf_cset_set (map (subst_cb Z P) F ++ E) A).
+    intros a aInA.
+    destruct (H a aInA)...
+    ** left. destruct H0. apply binds_app_1 in H0. destruct H0.
+       *** eexists.
+           apply binds_app_2.
+           eapply binds_map_2 with (f := subst_cb Z P) in H0...
+       *** analyze_binds H0...
+    ** right. destruct H0. apply binds_app_1 in H0. destruct H0.
+      *** eexists.
+          apply binds_app_2.
+          eapply binds_map_2 with (f := subst_cb Z P) in H0...
+      *** analyze_binds H0...
+          rewrite <- AtomSetFacts.not_mem_iff in *.
+          AtomSetDecide.fsetdec.
+Qed.
+
+(*
+Lemma subst_cs_open_ss_rec : forall k U Z P T,
+  open_ss_rec k (subst_cs Z P U) (subst_cs Z P T) = subst_cs Z P (open_ss_rec k U T)
+with subst_ct_open_st_rec : forall k U Z P T,
+  open_st_rec k (subst_cs Z P U) (subst_ct Z P T) = subst_ct Z P (open_st_rec k U T).
+Proof with eauto.
+-----
+  clear subst_cs_open_ss_rec.
+  intros *.
+  induction T; simpl in *; f_equal...
+  destruct (k == n)...
+-----
+  clear subst_ct_open_st_rec.
+  intros *.
+  induction T; simpl in *; f_equal...
+Qed.
+
+Lemma subst_ct_open_st_var : forall (X : atom) Z P T,
+  open_st (subst_ct Z P T) X = subst_ct Z P (open_st T X).
+Proof with eauto.
+  intros. unfold open_st.
+  assert (shp_fvar X = subst_cs Z P X) by eauto.
+  rewrite H. eapply subst_ct_open_st_rec.
+Qed.
+ *)
+
+Lemma wf_shp_subst_cbc : forall F Q E Z P T,
+  wf_shp (F ++ Z ~ bind_sub_cap Q ++ E) T ->
+  wf_cap E P ->
+  uniq (map (subst_cb Z P) F ++ E) ->
+  wf_shp (map (subst_cb Z P) F ++ E) (subst_cs Z P T)
+with wf_typ_subst_cbc : forall F Q E Z P T,
+  wf_typ (F ++ Z ~ bind_sub_cap Q ++ E) T ->
+  wf_cap E P ->
+  uniq (map (subst_cb Z P) F ++ E) ->
+  wf_typ (map (subst_cb Z P) F ++ E) (subst_ct Z P T).
+Proof with simpl_env; eauto using wf_typ_weaken_head, type_from_wf_typ,
+  shape_from_wf_shp.
+-----
+  clear wf_shp_subst_cbc.
+  intros * WfShp WfCap Uniq.
+  remember (F ++ Z ~ bind_sub_cap Q ++ E) as G.
+  generalize dependent F.
+  induction WfShp; intros F EQ Ok; subst...
+  - analyze_binds H...
+    + eapply wf_shp_fvar.
+      eapply binds_map_2 with (f := subst_cb Z P) in BindsTac...
+    + eapply wf_shp_fvar.
+      eapply binds_app_3...
+  - pick fresh X and apply wf_shp_arrow... fold subst_ct.
+    replace (cset_fvar X) with (subst_cc Z P (cset_fvar X))...
+    rewrite <- subst_ct_open_ct.
+    rewrite_env ((map (subst_cb Z P) (X ~ bind_typ T1 ++ F)) ++ E).
+    eapply wf_typ_subst_cbc...
+    eapply capture_from_wf_cap...
+    repeat (simpl; unfold subst_cc)...
+    destruct (AtomSetImpl.mem Z (singleton X)) eqn:ZX...
+    exfalso; rewrite <- AtomSetFacts.mem_iff in *. AtomSetDecide.fsetdec.
+  - pick fresh X and apply wf_shp_sall...
+    fold subst_cs subst_ct.
+    rewrite_env ((map (subst_cb Z P) (X ~ bind_sub_shp S ++ F)) ++ E).
+    rewrite <- subst_ct_open_st_var...
+    rewrite <- map_one. rewrite <- app_assoc. rewrite <- map_app.
+    eapply wf_typ_subst_cbc...
+  - pick fresh X and apply wf_shp_call;
+      fold subst_cs subst_ct...
+    + inversion H; subst; repeat (simpl; unfold subst_cc)...
+
+      destruct (AtomSetImpl.mem Z A) eqn:ZinA; subst...
+      * inversion WfCap; subst; autorewrite with core...
+        constructor; intros.
+        rewrite <- AtomSetFacts.mem_iff in ZinA.
+        rewrite AtomSetFacts.union_iff in H3; destruct H3...
+          assert (a `in` A) by AtomSetDecide.fsetdec.
+          destruct (H1 a)...
+          destruct (H5) as [U Bindsa].
+          analyze_binds Bindsa...
+          eapply binds_map_2
+            with (f := subst_cb Z (cset_set A0 {}N))
+            in BindsTac.
+          left; eexists; apply binds_app_2...
+          exfalso; AtomSetDecide.fsetdec.
+          destruct (H5) as [V Bindsa].
+          analyze_binds Bindsa...
+          eapply binds_map_2
+            with (f := subst_cb Z (cset_set A0 {}N))
+            in BindsTac.
+          right; eexists; apply binds_app_2...
+          destruct (H2 a)...
+          destruct (H4) as [U BindsU]...
+          destruct (H4) as [V BindsV]...
+      * constructor; intros.
+        rewrite <- AtomSetFacts.not_mem_iff in ZinA.
+        destruct (H1 a)...
+        destruct (H3) as [U Bindsa]...
+        analyze_binds Bindsa...
+        eapply binds_map_2
+          with (f := subst_cb Z P)
+          in BindsTac.
+        left; eexists; apply binds_app_2...
+        destruct (H3) as [V Bindsa]...
+        analyze_binds Bindsa...
+        eapply binds_map_2
+          with (f := subst_cb Z P)
+          in BindsTac.
+        right; eexists...
+    + rewrite subst_ct_open_ct_var...
+      rewrite_env ((map (subst_cb Z P) ((X ~ bind_sub_cap C) ++ F)) ++ E).
+      eapply wf_typ_subst_cbc...
+      eapply capture_from_wf_cap... 
+-----
+  clear wf_typ_subst_cbc.
+  intros * WfTyp WfCap Uniq.
+  remember (F ++ Z ~ bind_sub_cap Q ++ E) as G.
+  generalize dependent F.
+  induction WfTyp; intros F EQ Ok; subst...
+  simpl subst_ct... constructor...
+  eapply wf_cap_subst_cbc...
+Qed.
+
+
+Lemma wf_shp_subst_cbt : forall F Q E Z P T,
+  wf_shp (F ++ Z ~ bind_typ Q ++ E) T ->
+  wf_cap E P ->
+  uniq (map (subst_cb Z P) F ++ E) ->
+  wf_shp (map (subst_cb Z P) F ++ E) (subst_cs Z P T)
+with wf_typ_subst_cbt : forall F Q E Z P T,
+  wf_typ (F ++ Z ~ bind_typ Q ++ E) T ->
+  wf_cap E P ->
+  uniq (map (subst_cb Z P) F ++ E) ->
+  wf_typ (map (subst_cb Z P) F ++ E) (subst_ct Z P T).
+Proof with simpl_env; eauto using wf_typ_weaken_head, type_from_wf_typ,
+  shape_from_wf_shp.
+-----
+  clear wf_shp_subst_cbt.
+  intros * WfShp WfCap Uniq.
+  remember (F ++ Z ~ bind_typ Q ++ E) as G.
+  generalize dependent F.
+  induction WfShp; intros F EQ Ok; subst...
+  - analyze_binds H...
+    + eapply wf_shp_fvar.
+      eapply binds_map_2 with (f := subst_cb Z P) in BindsTac...
+    + eapply wf_shp_fvar.
+      eapply binds_app_3...
+  - pick fresh X and apply wf_shp_arrow... fold subst_ct.
+    replace (cset_fvar X) with (subst_cc Z P (cset_fvar X))...
+    rewrite <- subst_ct_open_ct...
+    rewrite_env ((map (subst_cb Z P) (X ~ bind_typ T1 ++ F)) ++ E).
+    eapply wf_typ_subst_cbt...
+    eapply capture_from_wf_cap...
+    repeat (simpl; unfold subst_cc); destruct (AtomSetImpl.mem Z (singleton X)) eqn:ZinX...
+    exfalso; rewrite <- AtomSetFacts.mem_iff in ZinX. AtomSetDecide.fsetdec.  
+  - pick fresh X and apply wf_shp_sall...
+    fold subst_cs subst_ct.
+    rewrite_env ((map (subst_cb Z P) (X ~ bind_sub_shp S ++ F)) ++ E).
+    rewrite <- subst_ct_open_st_var...
+    rewrite <- map_one. rewrite <- app_assoc. rewrite <- map_app.
+    eapply wf_typ_subst_cbt...
+  - pick fresh X and apply wf_shp_call;
+      fold subst_cs subst_ct...
+    + inversion H; subst;  repeat (simpl; unfold subst_cc)...
+      destruct (AtomSetImpl.mem Z A) eqn:ZinA; subst...
+      * inversion WfCap; subst; autorewrite with core...
+        constructor; intros.
+        rewrite <- AtomSetFacts.mem_iff in ZinA.
+        rewrite AtomSetFacts.union_iff in H3; destruct H3...
+          assert (a `in` A) by AtomSetDecide.fsetdec.
+          destruct (H1 a)...
+          destruct (H5) as [U Bindsa].
+          analyze_binds Bindsa...
+          eapply binds_map_2
+            with (f := subst_cb Z (cset_set A0 {}N))
+            in BindsTac.
+          left; eexists; apply binds_app_2...
+          destruct (H5) as [V Bindsa].
+          analyze_binds Bindsa...
+          eapply binds_map_2
+            with (f := subst_cb Z (cset_set A0 {}N))
+            in BindsTac.
+          right; eexists; apply binds_app_2...
+          exfalso; AtomSetDecide.fsetdec.
+          destruct (H2 a)...
+          destruct (H4) as [U BindsU]...
+          destruct (H4) as [V BindsV]...
+      * constructor; intros.
+        rewrite <- AtomSetFacts.not_mem_iff in ZinA.
+        destruct (H1 a)...
+        destruct (H3) as [U Bindsa]...
+        analyze_binds Bindsa...
+        eapply binds_map_2
+          with (f := subst_cb Z P)
+          in BindsTac.
+        left; eexists; apply binds_app_2...
+        destruct (H3) as [V Bindsa]...
+        analyze_binds Bindsa...
+        eapply binds_map_2
+          with (f := subst_cb Z P)
+          in BindsTac.
+        right; eexists...
+    + rewrite subst_ct_open_ct_var...
+      rewrite_env ((map (subst_cb Z P) ((X ~ bind_sub_cap C) ++ F)) ++ E).
+      eapply wf_typ_subst_cbt...
+      eapply capture_from_wf_cap... 
+-----
+  clear wf_typ_subst_cbt.
+  intros * WfTyp WfCap Uniq.
+  remember (F ++ Z ~ bind_typ Q ++ E) as G.
+  generalize dependent F.
+  induction WfTyp; intros F EQ Ok; subst...
+  simpl subst_ct... constructor...
+  eapply wf_cap_subst_cbt...
+Qed.
+
+Lemma wf_shp_open : forall E U T1 T2,
   uniq E ->
-  wf_typ E (typ_all T1 T2) ->
-  wf_typ E U ->
-  wf_typ E (open_tt T2 U).
+  wf_shp E (shp_sall T1 T2) ->
+  wf_shp E U ->
+  wf_typ E (open_st T2 U).
 Proof with simpl_env; eauto.
   intros E U T1 T2 Ok WA WU.
   inversion WA; subst.
   pick fresh X.
-  rewrite (subst_tt_intro X)...
-  rewrite_env (map (subst_tb X U) empty ++ E).
-  eapply wf_typ_subst_tb...
+  rewrite (subst_st_intro X)...
+  rewrite_env (map (subst_sb X U) empty ++ E).
+  eapply wf_typ_subst_sbs...
 Qed.
+
+Lemma wf_cap_open : forall E U T1 T2,
+  uniq E ->
+  wf_shp E (shp_call T1 T2) ->
+  wf_cap E U ->
+  wf_typ E (open_ct T2 U).
+Proof with simpl_env; eauto.
+  intros E U T1 T2 Ok WA WU.
+  inversion WA; subst.
+  pick fresh X.
+  rewrite (subst_ct_intro X)...
+  rewrite_env (map (subst_cb X U) empty ++ E).
+  eapply wf_typ_subst_cbc...
+Qed.
+
+Lemma wf_cap_open_expr : forall E U T1 T2,
+  uniq E ->
+  wf_shp E (shp_arrow T1 T2) ->
+  wf_cap E U ->
+  wf_typ E (open_ct T2 U).
+Proof with simpl_env; eauto.
+  intros E U T1 T2 Ok WA WU.
+  inversion WA; subst.
+  pick fresh X.
+  rewrite (subst_ct_intro X)...
+  rewrite_env (map (subst_cb X U) empty ++ E).
+  eapply wf_typ_subst_cbt with (Q := T1)...
+Qed.
+
 
 
 (* ********************************************************************** *)
@@ -161,6 +1012,35 @@ Proof with auto using wf_typ_weaken_head.
   injection BindsTacVal; intros; subst...
 Qed.
 
+Lemma wf_shp_from_binds_shp : forall x U E,
+  wf_env E ->
+  binds x (bind_sub_shp U) E ->
+  wf_shp E U.
+Proof with auto using wf_shp_weaken_head.
+  induction 1; intros J; analyze_binds J...
+  injection BindsTacVal; intros; subst...
+Qed.
+
+Lemma wf_cap_from_binds_cap : forall x U E,
+  wf_env E ->
+  binds x (bind_sub_cap U) E ->
+  wf_cap E U.
+Proof with auto using wf_cap_weaken_head.
+  induction 1; intros J; analyze_binds J...
+  injection BindsTacVal; intros; subst...
+Qed.
+
+Lemma wf_cap_from_binds_typ : forall x Sh U E,
+  wf_env E ->
+  binds x (bind_typ (pair Sh U)) E ->
+  wf_cap E U.
+Proof with auto using wf_cap_weaken_head.
+  induction 1; intros J; analyze_binds J...
+  injection BindsTacVal; intros; subst...
+  inversion H0...
+Qed.
+
+
 Lemma wf_typ_from_wf_env_typ : forall x T E,
   wf_env (x ~ bind_typ T ++ E) ->
   wf_typ E T.
@@ -168,9 +1048,16 @@ Proof.
   intros x T E H. inversion H; auto.
 Qed.
 
-Lemma wf_typ_from_wf_env_sub : forall x T E,
-  wf_env (x ~ bind_sub T ++ E) ->
-  wf_typ E T.
+Lemma wf_shp_from_wf_env_sub_shp : forall x T E,
+  wf_env (x ~ bind_sub_shp T ++ E) ->
+  wf_shp E T.
+Proof.
+  intros x T E H. inversion H; auto.
+Qed.
+
+Lemma wf_cap_from_wf_env_sub_cap : forall x T E,
+  wf_env (x ~ bind_sub_cap T ++ E) ->
+  wf_cap E T.
 Proof.
   intros x T E H. inversion H; auto.
 Qed.
@@ -182,167 +1069,595 @@ Qed.
 (** These properties are analogous to the properties that we need to
     show for the subtyping and typing relations. *)
 
-Lemma wf_env_narrowing : forall V E F U X,
-  wf_env (F ++ X ~ bind_sub V ++ E) ->
-  wf_typ E U ->
-  wf_env (F ++ X ~ bind_sub U ++ E).
-Proof with eauto using wf_typ_narrowing.
+Lemma wf_env_narrowing_cap : forall V E F U X,
+  wf_env (F ++ X ~ bind_sub_cap V ++ E) ->
+  wf_cap E U ->
+  wf_env (F ++ X ~ bind_sub_cap U ++ E).
+Proof with eauto using wf_cap_narrowing_cap.
   induction F; intros U X Wf_env Wf;
     inversion Wf_env; subst; simpl_env in *...
+    * apply (wf_env_sub_shp (F ++ X ~ bind_sub_cap U ++ E) X0 Sh)... 
+      apply (wf_shp_narrowing_cap V _ _ _ _ _).
+      apply H2.
+    * apply wf_env_typ...
+      apply (wf_typ_narrowing_cap V _ _ _ _ _).
+      apply H2.
 Qed.
 
-Lemma wf_env_strengthening : forall x T E F,
-  wf_env (F ++ x ~ bind_typ T ++ E) ->
-  wf_env (F ++ E).
-Proof with eauto using wf_typ_strengthening.
-  induction F; intros Wf_env; inversion Wf_env; subst; simpl_env in *...
+Lemma wf_env_narrowing_shp : forall V E F U X,
+  wf_env (F ++ X ~ bind_sub_shp V ++ E) ->
+  wf_shp E U ->
+  wf_env (F ++ X ~ bind_sub_shp U ++ E).
+Proof with eauto using wf_cap_narrowing_cap.
+  induction F; intros U X Wf_env Wf;
+    inversion Wf_env; subst; simpl_env in *...
+    * apply (wf_env_sub_shp (F ++ X ~ bind_sub_shp U ++ E) X0 Sh)... 
+      apply (wf_shp_narrowing_shp V _ _ _ _ _).
+      apply H2.
+    * apply wf_env_sub_cap...
+      apply (wf_cap_narrowing_shp V _ _ _ _ _).
+      apply H2.
+    * apply wf_env_typ...
+      apply (wf_typ_narrowing_shp V _ _ _ _ _).
+      apply H2.
+Qed.
+
+Lemma wf_env_narrowing_typ : forall V E F U X,
+  wf_env (F ++ X ~ bind_typ V ++ E) ->
+  wf_typ E U ->
+  wf_env (F ++ X ~ bind_typ U ++ E).
+Proof with eauto using wf_cap_narrowing_cap.
+  induction F; intros U X Wf_env Wf;
+    inversion Wf_env; subst; simpl_env in *...
+    * apply (wf_env_sub_shp (F ++ X ~ bind_typ U ++ E) X0 Sh)...
+      apply (wf_shp_narrowing_typ V)...
+    * apply (wf_env_sub_cap (F ++ X ~ bind_typ U ++ E) X0 C)...
+      apply (wf_cap_narrowing_typ V)...
+    * apply (wf_env_typ (F ++ X ~ bind_typ U ++ E) x T)...
+      apply (wf_typ_narrowing_typ V)...
+Qed.
+
+Lemma wf_env_subst_sbs : forall Q Z P E F,
+  wf_env (F ++ Z ~ bind_sub_shp Q ++ E) ->
+  wf_shp E P ->
+  wf_env (map (subst_sb Z P) F ++ E).
+Proof with eauto 6 using wf_shp_subst_sbs.
+  induction F; intros Wf_env WP; simpl_env;
+    inversion Wf_env; simpl_env in *; simpl subst_sb...
+    * apply wf_env_sub_cap...
+      apply (wf_cap_subst_sbs _ Q _ _ _ _)...
+    * apply wf_env_typ...
+      apply (wf_typ_subst_sbs _ Q _ _ _)...
+Qed.
+
+Lemma wf_env_subst_cbc : forall Q Z P E F,
+  wf_env (F ++ Z ~ bind_sub_cap Q ++ E) ->
+  wf_cap E P ->
+  wf_env (map (subst_cb Z P) F ++ E).
+Proof with eauto 6 using wf_cap_subst_cbc.
+  induction F; intros Wf_env WP; simpl_env;
+    inversion Wf_env; simpl_env in *; simpl subst_cb...
+    * apply wf_env_sub_shp...
+      apply (wf_shp_subst_cbc _ Q _ _ _ _)...
+    * apply wf_env_typ...
+      apply (wf_typ_subst_cbc _ Q _ _ _)...
 Qed.
 
 Lemma wf_env_subst_tb : forall Q Z P E F,
-  wf_env (F ++ Z ~ bind_sub Q ++ E) ->
-  wf_typ E P ->
-  wf_env (map (subst_tb Z P) F ++ E).
-Proof with eauto 6 using wf_typ_subst_tb.
+  wf_env (F ++ Z ~ bind_typ Q ++ E) ->
+  wf_cap E P ->
+  wf_env (map (subst_cb Z P) F ++ E).
+Proof with eauto 6 using wf_shp_subst_cbt, wf_cap_subst_cbt, wf_typ_subst_cbt.
   induction F; intros Wf_env WP; simpl_env;
-    inversion Wf_env; simpl_env in *; simpl subst_tb...
+    inversion Wf_env; simpl_env in *; simpl subst_cb...
 Qed.
 
 
 (* ********************************************************************** *)
 (** * #<a name="subst"></a># Environment is unchanged by substitution for a fresh name *)
 
-Lemma notin_fv_tt_open : forall (Y X : atom) T,
-  X `notin` fv_tt (open_tt T Y) ->
-  X `notin` fv_tt T.
+(*** TODO: generalize for all k in opening, and then prove *)
+Lemma notin_fv_ss_open_cs_rec : forall (Y X : atom) k T,
+  X `notin` fv_ss (open_cs_rec k (cset_fvar Y) T) ->
+  X `notin` fv_ss T
+with notin_fv_st_open_ct_rec : forall (Y X : atom) k T,
+  X `notin` fv_st (open_ct_rec k (cset_fvar Y) T) ->
+  X `notin` fv_st T.
 Proof.
- intros Y X T. unfold open_tt.
- generalize 0.
- induction T; simpl; intros k Fr; eauto.
+-----   
+  clear notin_fv_ss_open_cs_rec.
+  intros Y X k T. unfold open_cs, open_ct in *.
+  generalize dependent k.
+  induction T; simpl; intros k Fr; eauto.
+-----
+  clear notin_fv_st_open_ct_rec.
+  intros Y X k T. unfold open_cs, open_ct in *.
+  generalize dependent k.
+  induction T; simpl; intros k Fr; eauto. 
 Qed.
 
-Lemma notin_fv_wf : forall E (X : atom) T,
-  wf_typ E T ->
+Lemma notin_fv_st_open_ct : forall (Y X : atom) T,
+  X `notin` fv_st (open_ct T (cset_fvar Y)) ->
+  X `notin` fv_st T.
+Proof with eauto.
+  intros; unfold open_ct.
+  eapply notin_fv_st_open_ct_rec...
+Qed.
+
+Lemma notin_fv_ss_open_ss_rec : forall (Y X : atom) k T,
+  X `notin` fv_ss (open_ss_rec k Y T) ->
+  X `notin` fv_ss T
+with notin_fv_st_open_st_rec : forall (Y X : atom) k T,
+  X `notin` fv_st (open_st_rec k Y T) ->
+  X `notin` fv_st T.
+Proof.
+-----   
+  clear notin_fv_ss_open_ss_rec.
+  intros Y X k T. unfold open_ss, open_st in *.
+  generalize dependent k.
+  induction T; simpl; intros k Fr; eauto.
+-----
+  clear notin_fv_st_open_st_rec.
+  intros Y X k T. unfold open_cs, open_ct in *.
+  generalize dependent k.
+  induction T; simpl; intros k Fr; eauto.
+Qed.
+
+Lemma notin_fv_st_open_st : forall (Y X : atom) T,
+  X `notin` fv_st (open_st T Y) ->
+  X `notin` fv_st T.
+Proof with eauto.
+  intros; unfold open_st.
+  eapply notin_fv_st_open_st_rec...
+Qed.
+
+
+Lemma notin_fv_cs_open_ss_rec : forall (Y X : atom) k T,
+  X `notin` fv_cs (open_ss_rec k Y T) ->
+  X `notin` fv_cs T
+with notin_fv_ct_open_st_rec : forall (Y X : atom) k T,
+  X `notin` fv_ct (open_st_rec k Y T) ->
+  X `notin` fv_ct T.
+Proof.
+-----   
+  clear notin_fv_cs_open_ss_rec.
+  intros Y X k T. unfold open_ss, open_st in *.
+  generalize dependent k.
+  induction T; simpl; intros k Fr; eauto.
+-----
+  clear notin_fv_ct_open_st_rec.
+  intros Y X k T. unfold open_cs, open_ct in *.
+  generalize dependent k.
+  induction T; simpl; intros k Fr; eauto.
+Qed.
+
+Lemma notin_fv_ct_open_st : forall (Y X : atom) T,
+  X `notin` fv_ct (open_st T Y) ->
+  X `notin` fv_ct T.
+Proof with eauto.
+  intros; unfold open_st.
+  eapply notin_fv_ct_open_st_rec...
+Qed.
+
+
+Lemma notin_fv_cs_open_cs_rec : forall (Y X : atom) k T,
+  X `notin` fv_cs (open_cs_rec k (cset_fvar Y) T) ->
+  X `notin` fv_cs T
+with notin_fv_ct_open_ct_rec : forall (Y X : atom) k T,
+  X `notin` fv_ct (open_ct_rec k (cset_fvar Y) T) ->
+  X `notin` fv_ct T.
+Proof with eauto; try solve csetdec.
+-----   
+  clear notin_fv_cs_open_cs_rec.
+  intros Y X k T. unfold open_cs, open_st in *.
+  generalize dependent k.
+  induction T; simpl; intros k Fr; eauto.
+  unshelve epose proof (notin_fv_ct_open_ct_rec Y X (S k) t _)...
+  csetdec.
+  unfold open_cc_rec in Fr; destruct c eqn:HC; subst; simpl fv_cc...
+  csetdec.
+  destruct (NatSetImpl.mem k t1); simpl in *...
+-----
+  clear notin_fv_ct_open_ct_rec.
+  intros Y X k T. unfold open_cs, open_ct in *.
+  generalize dependent k.
+  induction T; simpl; intros k Fr; eauto.
+  unshelve epose proof (notin_fv_cs_open_cs_rec Y X k s _)...
+  unfold open_cc_rec in Fr; destruct c eqn:HC; subst; simpl fv_cc...
+  csetdec.
+  destruct (NatSetImpl.mem k t0); simpl in *...
+Qed.
+
+Lemma notin_fv_ct_open_ct : forall (Y X : atom) T,
+  X `notin` fv_ct (open_ct T (cset_fvar Y)) ->
+  X `notin` fv_ct T.
+Proof with eauto; try solve csetdec.
+  intros.
+  eapply notin_fv_ct_open_ct_rec...
+Qed.
+
+(*
+Lemma notin_fv_ss_open_sc : forall (Y X : atom) T,
+  X `notin` fv_sc (open_cc T (cset_fvar Y)) ->
+  X `notin` fv_sc T.
+Proof.
+ intros Y X T. unfold open_cc.
+ generalize 0.
+ induction T; simpl; intros k Fr; eauto.
+ destruct (NatSetImpl.mem k t0)...
+ * unfold fv_sc in Fr. auto.
+ * auto.
+Qed.
+ *)
+
+Lemma notin_fv_wf_cap : forall E (X : atom) T,
+  wf_cap E T ->
   X `notin` dom E ->
-  X `notin` fv_tt T.
+   X `notin` fv_cc T.
 Proof with auto.
   intros E X T Wf_typ.
   induction Wf_typ; intros Fr; simpl...
-  Case "wf_typ_var".
-    assert (X0 `in` (dom E))...
-    eapply binds_In; eauto.
-    assert (X <> X0) by fsetdec. fsetdec.
-  Case "wf_typ_all".
-    apply notin_union...
-    pick fresh Y.
-    apply (notin_fv_tt_open Y)...
+  intro xInA. destruct (H X xInA); destruct H0. 
+    ** apply (binds_dom_contradiction _ X (bind_sub_cap x) E)...
+    ** apply (binds_dom_contradiction _ X (bind_typ x) E)...
 Qed.
 
-Lemma map_subst_tb_id : forall G Z P,
+Lemma notin_fv_wf_shp : forall E (X : atom) T,
+  wf_shp E T ->
+  X `notin` dom E ->
+  X `notin` fv_ss T /\ X `notin` fv_cs T
+with notin_fv_wf_typ : forall E (X : atom) T,
+  wf_typ E T ->
+  X `notin` dom E ->
+  X `notin` fv_st T /\ X `notin` fv_ct T.
+Proof with auto.
+  ----- clear notin_fv_wf_shp.
+        intros E X T Wf_typ.
+        induction Wf_typ; intros Fr; simpl...
+        * split; auto. destruct (X == x)...
+          rewrite e in *.
+          destruct (binds_dom_contradiction _ x (bind_sub_shp U) E)...
+        * split; apply union_rewrite; split.
+          ** apply (notin_fv_wf_typ E _ T1)...
+          ** pick fresh y.
+             eapply notin_fv_wf_typ with (X := X) in H0
+              as [FrOpen FrCaptOpen]...
+             eapply notin_fv_st_open_ct...
+          ** apply (notin_fv_wf_typ E _ T1)...
+          ** pick fresh y.
+             eapply notin_fv_wf_typ with (X := X) in H0
+              as [FrOpen FrCaptOpen]...
+             eapply notin_fv_ct_open_ct...
+        * split; apply union_rewrite; split.
+          ** apply (IHWf_typ Fr)...
+          ** pick fresh Y. 
+             eapply notin_fv_wf_typ with (X := X) in H
+              as [FrOpen FrCaptOpen]...
+             eapply notin_fv_st_open_st... 
+          ** apply (IHWf_typ Fr)...
+          ** pick fresh Y. 
+             eapply notin_fv_wf_typ with (X := X) in H
+              as [FrOpen FrCaptOpen]...
+             eapply notin_fv_ct_open_st...
+        * split... 
+          ** pick fresh Y.
+             eapply notin_fv_wf_typ with (X := X) in H0
+                as [FrOpen FrCaptOpen]...
+             eapply notin_fv_st_open_ct...
+          ** unshelve epose proof (notin_fv_wf_cap E X C _ _)...
+             apply union_rewrite; split...
+             pick fresh Y.
+             eapply notin_fv_wf_typ with (X := X) in H0
+              as [FrOpen FrCaptOpen]...
+             eapply notin_fv_ct_open_ct...          
+-----
+  clear notin_fv_wf_typ.
+  intros E X T Wf_typ.
+  induction Wf_typ; intros Fr; simpl...
+  split...
+  unshelve epose proof (notin_fv_wf_shp E X S)...
+  apply union_rewrite; split...
+  unshelve epose proof (notin_fv_wf_shp E X S)...
+  unshelve epose proof (notin_fv_wf_cap E X C)...
+Qed.
+
+Lemma map_subst_sb_id : forall G Z P,
   wf_env G ->
   Z `notin` dom G ->
-  G = map (subst_tb Z P) G.
+  G = map (subst_sb Z P) G.
 Proof with auto.
   intros G Z P H.
   induction H; simpl; intros Fr; simpl_env...
   rewrite <- IHwf_env...
-    rewrite <- subst_tt_fresh... eapply notin_fv_wf; eauto.
+    rewrite <- subst_ss_fresh... eapply notin_fv_wf_shp; eauto.
   rewrite <- IHwf_env...
-    rewrite <- subst_tt_fresh... eapply notin_fv_wf; eauto.
+    rewrite <- subst_st_fresh... f_equal... destruct (notin_fv_wf_typ E Z T)...
+Qed.
+
+
+Lemma map_subst_cb_id : forall G Z P,
+  wf_env G ->
+  Z `notin` dom G ->
+  G = map (subst_cb Z P) G.
+Proof with auto.
+  intros G Z P H.
+  induction H; simpl; intros Fr; simpl_env...
+  rewrite <- IHwf_env...
+    rewrite <- subst_cs_fresh... eapply notin_fv_wf_shp; eauto.
+  rewrite <- IHwf_env...
+    rewrite <- subst_cc_fresh... apply (notin_fv_wf_cap E Z C)...
+  rewrite <- IHwf_env...
+    rewrite <- subst_ct_fresh... destruct (notin_fv_wf_typ E Z T)... 
 Qed.
 
 
 (* ********************************************************************** *)
 (** * #<a name="regularity"></a># Regularity of relations *)
 
-Lemma sub_regular : forall E S T,
-  sub E S T ->
-  wf_env E /\ wf_typ E S /\ wf_typ E T.
+Lemma sub_cap_regular : forall E S T,
+  sub_cap E S T ->
+  wf_env E /\ wf_cap E S /\ wf_cap E T.
 Proof with simpl_env; try solve [auto | intuition auto].
   intros E S T H.
   induction H...
-  Case "sub_trans_tvar".
-    intuition eauto.
-  Case "sub_all".
-    repeat split...
-    SCase "Second of original three conjuncts".
-      pick fresh Y and apply wf_typ_all...
-      destruct (H1 Y)...
-      rewrite_env (empty ++ Y ~ bind_sub S1 ++ E).
-      apply (wf_typ_narrowing T1)...
-    SCase "Third of original three conjuncts".
-      pick fresh Y and apply wf_typ_all...
-      destruct (H1 Y)...
+  * split... split...
+    remember (cset_set ys {}N)...
+    destruct H0 eqn:h0...
+    ** discriminate Heqc.
+    ** apply wf_cset_set...
+       intros a aInx...
+       inversion Heqc...
+       replace a with x by AtomSetDecide.fsetdec.
+       apply (o x)...
+       rewrite H3...
+  * split... split...
+    inversion IHsub_cap. inversion H2.
+    remember (cset_set ys {}N)...
+    apply wf_cset_set...
+    intros a aInx...
+    left. eapply ex_intro...
+    replace a with x by AtomSetDecide.fsetdec.
+    apply H0...
+  * split... split...
+    ** apply wf_cset_set...
+       intros a aInx.
+       replace a with x by AtomSetDecide.fsetdec.
+       right.
+       eapply ex_intro.
+       apply H0.
+Qed.
+
+Lemma sub_shp_regular : forall E S T,
+  sub_shp E S T ->
+  wf_env E /\ wf_shp E S /\ wf_shp E T
+with sub_typ_regular : forall E S T,
+  sub_typ E S T ->
+  wf_env E /\ wf_typ E S /\ wf_typ E T.
+Proof with simpl_env; try solve [auto | intuition auto].
+  ----- clear sub_shp_regular.
+        intros E S T H.
+        induction H...
+        * inversion IHsub_shp. inversion H2. split; eauto.
+        * split.
+          ** destruct (sub_typ_regular E T1 S1)...
+          ** split.
+             *** eapply wf_shp_arrow. destruct (sub_typ_regular E T1 S1)...
+                 intros X XnInL.
+                 eapply sub_typ_regular in H0 as [WfEnv [WfTypL WfTypR]]...
+                 rewrite_env (empty ++ X ~ bind_typ S1 ++ E).
+                 eapply wf_typ_narrowing_typ with (V := T1)...
+             *** eapply wf_shp_arrow with (L := L). destruct (sub_typ_regular E T1 S1)...
+                 intros X XnInL.
+                 unshelve epose proof (sub_typ_regular _ _ _ (H0 X XnInL))...
+        * split.
+          ** destruct IHsub_shp...
+          ** split; apply (wf_shp_sall L _ _ _).
+             *** destruct IHsub_shp. destruct H2. apply H3.
+             *** intros X xnInL. destruct ((sub_typ_regular _ _ _) (H0 X xnInL))... 
+                 destruct H2...
+                 apply (wf_typ_narrowing_shp T1 S1 (open_st S2 X) E empty X)...
+             *** destruct IHsub_shp. destruct H2. apply H2.
+             *** intros X xnInL. destruct ((sub_typ_regular _ _ _) (H0 X xnInL))...
+        * split.
+          ** destruct (sub_cap_regular E T1 S1)...
+          ** split; apply (wf_shp_call L _ _ _).
+             *** destruct (sub_cap_regular E T1 S1)...
+             *** intros X xnInL. destruct ((sub_typ_regular _ _ _) (H0 X xnInL))...
+                 destruct H2...
+                  apply (wf_typ_narrowing_cap T1 S1 (open_ct S2 (cset_fvar X)) E empty X)...
+             *** destruct (sub_cap_regular E T1 S1)...
+             *** intros X xnInL. destruct ((sub_typ_regular _ _ _) (H0 X xnInL))...
+  ----- clear sub_typ_regular.
+        intros E S T H.
+        induction H...
+        split; try split.
+        * destruct (sub_shp_regular E Sh1 Sh2)...
+        * apply wf_pair... destruct (sub_shp_regular E Sh1 Sh2)... destruct (sub_cap_regular E C1 C2)...
+        * apply wf_pair... destruct (sub_shp_regular E Sh1 Sh2)... destruct (sub_cap_regular E C1 C2)...
+Qed.
+
+Lemma fv_exp_cap_open_ee : forall e (k: nat) (x : atom) (Y : atom),
+  x `in` (fv_exp_for_cap e) ->
+  x `in` (fv_exp_for_cap (open_ee_rec k Y (cset_fvar Y) e)).
+Proof with eauto.
+  intros e k x Y Hxine. revert k.
+  induction e; intro k;simpl...
+  * unfold fv_exp_for_cap in Hxine.
+    AtomSetDecide.fsetdec.
+  * simpl in Hxine.
+    apply AtomSetImpl.union_1 in Hxine.
+    destruct Hxine.
+    ** apply AtomSetImpl.union_2...
+    ** apply AtomSetImpl.union_3...
+Qed.
+
+Lemma fv_exp_cap_open_se : forall e (k : nat) (x : atom) (Y : atom),
+  x `in` (fv_exp_for_cap e) ->
+  x `in` (fv_exp_for_cap (open_se_rec k Y e)).
+Proof with eauto.
+  intros e k x Y Hxine. revert k.
+  induction e; intro k; simpl...
+  simpl in Hxine.
+    apply AtomSetImpl.union_1 in Hxine.
+    destruct Hxine.
+    ** apply AtomSetImpl.union_2...
+    ** apply AtomSetImpl.union_3...
+Qed.
+
+Lemma fv_exp_cap_open_ce : forall e (k : nat) (x : atom) (Y : atom),
+  x `in` (fv_exp_for_cap e) ->
+  x `in` (fv_exp_for_cap (open_ce_rec k (cset_fvar Y) e)).
+Proof with eauto.
+  intros e k x Y Hxine. revert k.
+  induction e; intro k; simpl...
+  simpl in Hxine.
+    apply AtomSetImpl.union_1 in Hxine.
+    destruct Hxine.
+    ** apply AtomSetImpl.union_2...
+    ** apply AtomSetImpl.union_3...
+Qed.
+
+Lemma fv_exp_cap_bound_typing : forall E e (x : atom) T,
+  typing E e T ->
+  x `in` (fv_exp_for_cap e) ->
+  exists T, binds x (bind_typ T) E.
+Proof with eauto.
+  intros E e x T Ht xIn.
+  induction Ht; simpl in *...
+  * replace x with x0 by AtomSetDecide.fsetdec.
+    eapply ex_intro.
+    apply H0.
+  * pick fresh Y for (union L {{ x }}).
+    destruct (H0 Y)...
+    apply fv_exp_cap_open_ee...
+    eapply ex_intro...
+    analyze_binds H1...
+  * apply AtomSetImpl.union_1 in xIn.
+    destruct xIn...
+  * pick fresh Y for (union L {{ x }}).
+    destruct (H0 Y)...
+    apply fv_exp_cap_open_se...
+    eapply ex_intro...
+    analyze_binds H1...
+  * pick fresh Y for (union L {{ x }}).
+    destruct (H0 Y)...
+    apply fv_exp_cap_open_ce...
+    eapply ex_intro...
+    analyze_binds H1...
+Qed.
+
+Lemma typing_cap : forall E e T,
+  typing E e T ->
+  wf_cap E (cset_set (fv_exp_for_cap e) {}N).
+Proof with eauto using fv_exp_cap_bound_typing.
+  intros E e T Htyp.
+  induction Htyp...
+  * apply wf_cset_set...
+    intros a aInfv...
+    right...
+    pick fresh x for (union L {{ a }}).
+    apply union_rewrite in Fr. inversion Fr.
+    destruct (fv_exp_cap_bound_typing _ _ a _ (H x H1))...
+    apply fv_exp_cap_open_ee...
+    eapply ex_intro.
+    analyze_binds H3...
+  * apply wf_cset_set...
+    intros a aInfv...
+    right...
+    pick fresh x for (union L {{ a }}).
+    apply union_rewrite in Fr. inversion Fr.
+    destruct (fv_exp_cap_bound_typing _ _ a _ (H x H1))...
+    apply fv_exp_cap_open_se...
+    eapply ex_intro.
+    analyze_binds H3...
+  * apply wf_cset_set...
+    intros a aInfv...
+    right...
+    pick fresh x for (union L {{ a }}).
+    apply union_rewrite in Fr. inversion Fr.
+    destruct (fv_exp_cap_bound_typing _ _ a _ (H x H1))...
+    apply fv_exp_cap_open_ce...
+    eapply ex_intro.
+    analyze_binds H3...
 Qed.
 
 Lemma typing_regular : forall E e T,
   typing E e T ->
   wf_env E /\ expr e /\ wf_typ E T.
 Proof with simpl_env; try solve [auto | intuition auto].
-  intros E e T H; induction H...
-  Case "typing_var".
+  intros E e T H. assert (typing E e T) as Typing by assumption. induction H...
+  * repeat split...
+    eapply wf_typ_from_binds_typ in H0... inversion H0...
+    eapply wf_cset_set; intros.
+    replace a with x in * by AtomSetDecide.fsetdec; subst.
+    right... eexists; eassumption.
+  * pick fresh X. destruct (H0 X) as [Hok [J K]]...
     repeat split...
-    eauto using wf_typ_from_binds_typ.
-  Case "typing_abs".
-    pick fresh y.
-    destruct (H0 y) as [Hok [J K]]...
-    repeat split. inversion Hok...
-    SCase "Second of original three conjuncts".
-      pick fresh x and apply expr_abs.
-        eauto using type_from_wf_typ, wf_typ_from_wf_env_typ.
-        destruct (H0 x)...
-    SCase "Third of original three conjuncts".
-      apply wf_typ_arrow; eauto using wf_typ_from_wf_env_typ.
-      rewrite_env (empty ++ E).
-      eapply wf_typ_strengthening; simpl_env; eauto.
-  Case "typing_app".
+    - inversion Hok...
+    - apply expr_abs with (L := L)...
+      eapply type_from_wf_typ.
+      eapply wf_typ_from_binds_typ with (x := X) (E := X ~ bind_typ V ++ E)...
+      intros x Frx.
+      destruct (H0 x)...
+    - apply wf_shp_arrow with (L := L)...
+      inversion Hok...
+      intros X' FrX'...
+      destruct (H0 X')...
+    - unshelve epose proof (typing_cap _ _ _ Typing)...
+  * destruct (IHtyping1) as [WfEnv [Expr1 WfTyp]]...
+    destruct (IHtyping2) as [WfEnv2 [Expr2 WfTyp3]]...
     repeat split...
-    destruct IHtyping1 as [_ [_ K]].
-    inversion K...
-  Case "typing_tabs".
-    pick fresh Y.
-    destruct (H0 Y) as [Hok [J K]]...
-    inversion Hok; subst.
+    + constructor...
+      inversion WfTyp; subst...
+      inversion WfTyp3; subst...
+      eapply capture_from_wf_cap; eauto...
+    + inversion WfTyp; subst...
+      inversion H4; subst...
+      eapply wf_cap_open_expr with (T1 := (pair T1 C))...
+      inversion WfTyp3; subst...
+  * pick fresh Y. destruct (H0 Y) as [WfEnv [Expr WfTyp]]...
+    repeat split; eauto.
+    - inversion WfEnv...
+    - pick fresh Y' and apply expr_sabs...
+      eapply shape_from_wf_shp...
+      inversion WfEnv; subst; eauto...
+      destruct (H0 Y')...
+    - pick fresh Y' and apply wf_shp_sall.
+      inversion WfEnv...
+      destruct (H0 Y')...
+    - unshelve epose proof (typing_cap _ _ _ Typing)...
+  * destruct (IHtyping) as [WfEnv [Expr1 WfTyp1]]...
     repeat split...
-    SCase "Second of original three conjuncts".
-      pick fresh X and apply expr_tabs.
-        eauto using type_from_wf_typ, wf_typ_from_wf_env_sub...
+    - constructor...
+      destruct (sub_shp_regular _ _ _ H0) as [WfEnv1 [WfShp1 WfShp2]]...
+      eapply shape_from_wf_shp; eauto...
+    - inversion WfTyp1; inversion H4; subst...
+      eapply wf_shp_open with (T1 := Sh1)...
+      eapply sub_shp_regular with (S := Sh) (T := Sh1)...
+  * pick fresh Y.
+    destruct (H0 Y) as [WfEnv [Expr WfTyp]]...
+    repeat split...
+    - inversion WfEnv...
+    - apply expr_cabs with (L := L)...
+      + eapply capture_from_wf_cap.
+        eapply wf_cap_from_wf_env_sub_cap; eassumption...
+      + intros X Frx.
         destruct (H0 X)...
-    SCase "Third of original three conjuncts".
-      pick fresh Z and apply wf_typ_all...
-      destruct (H0 Z)...
-  Case "typing_tapp".
-    destruct (sub_regular _ _ _ H0) as [R1 [R2 R3]].
+    - apply wf_shp_call with (L := L)...
+      + eapply wf_cap_from_wf_env_sub_cap; eassumption...
+      + intros X' FrX'...
+        destruct (H0 X')... 
+    - unshelve epose proof (typing_cap _ _ _ Typing)...
+  * destruct IHtyping as [WfEnv [Expr WfTyp]]...
     repeat split...
-    SCase "Second of original three conjuncts".
-      apply expr_tapp...
-      eauto using type_from_wf_typ.
-    SCase "Third of original three conjuncts".
-      destruct IHtyping as [R1' [R2' R3']].
-      eapply wf_typ_open; eauto.
-  Case "typing_sub".
+    - constructor...
+      eapply capture_from_wf_cap.
+      eapply sub_cap_regular with (S := C) (T := C1); eassumption.
+    - inversion WfTyp. eapply wf_cap_open with (T1 := C1)...
+      eapply sub_cap_regular with (T := C1); eassumption.
+  * destruct IHtyping as [WfEnv [Expr WfTyp]]...
     repeat split...
-    destruct (sub_regular _ _ _ H0)...
-  Case "typing_let".
-    repeat split...
-    SCase "Second of original three conjuncts".
-      pick fresh y and apply expr_let...
-      destruct (H1 y) as [K1 [K2 K3]]...
-    SCase "Third of original three conjuncts".
-      pick fresh y.
-      destruct (H1 y) as [K1 [K2 K3]]...
-      rewrite_env (empty ++ E).
-      eapply wf_typ_strengthening; simpl_env; eauto.
-  Case "typing_case".
-    repeat split...
-    SCase "Second of original three conjuncts".
-      pick fresh x and apply expr_case...
-        destruct (H1 x) as [? [? ?]]...
-        destruct (H3 x) as [? [? ?]]...
-    SCase "Third of original three conjuncts".
-      pick fresh y.
-      destruct (H1 y) as [K1 [K2 K3]]...
-      rewrite_env (empty ++ E).
-      eapply wf_typ_strengthening; simpl_env; eauto.
+    eapply sub_typ_regular; eassumption...
 Qed.
 
 Lemma value_regular : forall e,
@@ -357,12 +1672,31 @@ Lemma red_regular : forall e e',
   expr e /\ expr e'.
 Proof with try solve [auto | intuition auto].
   intros e e' H.
-  induction H; assert(J := value_regular); split...
-  Case "red_abs".
-    inversion H. pick fresh y. rewrite (subst_ee_intro y)...
-  Case "red_tabs".
-    inversion H. pick fresh Y. rewrite (subst_te_intro Y)...
+  induction H; assert(J := value_regular); split; try apply expr_app...
+  * inversion H; subst.
+    pick fresh y. erewrite (subst_ee_intro)...
+  * inversion H; subst.
+    pick fresh Y. erewrite (subst_se_intro)...
+  * inversion H; subst.
+    pick fresh Y. erewrite (subst_ce_intro)...
 Qed.
+
+Lemma wf_cap_from_wf_typ : forall E S C,
+  wf_typ E (pair S C) ->
+  wf_cap E C.
+Proof with eauto.
+  intros.
+  inversion H...
+Qed.
+
+Lemma wf_shp_from_wf_typ : forall E S C,
+  wf_typ E (pair S C) ->
+  wf_shp E S.
+Proof with eauto.
+  intros.
+  inversion H...
+Qed.
+
 
 
 (* *********************************************************************** *)
@@ -394,23 +1728,67 @@ Qed.
 
 #[export] Hint Extern 1 (wf_env ?E) =>
   match goal with
-  | H: sub _ _ _ |- _ => apply (proj1 (sub_regular _ _ _ H))
+  | H: sub_typ _ _ _ |- _ => apply (proj1 (sub_typ_regular _ _ _ H))
+  | H: sub_shp _ _ _ |- _ => apply (proj1 (sub_shp_regular _ _ _ H))
+  | H: sub_cap _ _ _ |- _ => apply (proj1 (sub_cap_regular _ _ _ H))
   | H: typing _ _ _ |- _ => apply (proj1 (typing_regular _ _ _ H))
   end : core.
 
 #[export] Hint Extern 1 (wf_typ ?E ?T) =>
   match goal with
   | H: typing E _ T |- _ => apply (proj2 (proj2 (typing_regular _ _ _ H)))
-  | H: sub E T _ |- _ => apply (proj1 (proj2 (sub_regular _ _ _ H)))
-  | H: sub E _ T |- _ => apply (proj2 (proj2 (sub_regular _ _ _ H)))
+  | H: sub_typ E T _ |- _ => apply (proj1 (proj2 (sub_typ_regular _ _ _ H)))
+  | H: sub_typ E _ T |- _ => apply (proj2 (proj2 (sub_typ_regular _ _ _ H)))
+  end : core.
+
+#[export] Hint Extern 1 (wf_cap ?E ?C) =>
+  match goal with
+  | H: typing E _ (pair _ C)   |- _ => apply (wf_cap_from_wf_typ _ _ _ (proj2 (proj2 (typing_regular _ _ _ H))))
+  | H: sub_typ E (pair _ C) _  |- _ => apply (wf_cap_from_wf_typ _ _ _ (proj1 (proj2 (sub_typ_regular _ _ _ H))))
+  | H: sub_typ E _ (pair _ C)  |- _ => apply (wf_cap_from_wf_typ _ _ _ (proj2 (proj2 (sub_typ_regular _ _ _ H))))
+  end : core.
+
+#[export] Hint Extern 1 (wf_shp ?E ?T) =>
+  match goal with
+  | H: sub_shp E T _ |- _ => apply (proj1 (proj2 (sub_shp_regular _ _ _ H)))
+  | H: sub_shp E _ T |- _ => apply (proj2 (proj2 (sub_shp_regular _ _ _ H)))
+  end : core.
+
+#[export] Hint Extern 1 (wf_shp ?E ?S) =>
+  match goal with
+  | H: typing E _ (pair S _)    |- _ => apply (wf_shp_from_wf_typ _ _ _ (proj2 (proj2 (typing_regular _ _ _ H))))
+  | H: sub_typ E (pair S _) _   |- _ => apply (wf_shp_from_wf_typ _ _ _ (proj1 (proj2 (sub_typ_regular _ _ _ H))))
+  | H: sub_typ E _ (pair S _ )  |- _ => apply (wf_shp_from_wf_typ _ _ _ (proj2 (proj2 (sub_typ_regular _ _ _ H))))
+  end : core.
+
+#[export] Hint Extern 1 (wf_cap ?E ?T) =>
+  match goal with
+  | H: sub_cap E T _ |- _ => apply (proj1 (proj2 (sub_cap_regular _ _ _ H)))
+  | H: sub_cap E _ T |- _ => apply (proj2 (proj2 (sub_cap_regular _ _ _ H)))
   end : core.
 
 #[export] Hint Extern 1 (type ?T) =>
   let go E := apply (type_from_wf_typ E); auto in
   match goal with
   | H: typing ?E _ T |- _ => go E
-  | H: sub ?E T _ |- _ => go E
-  | H: sub ?E _ T |- _ => go E
+  | H: sub_typ ?E T _ |- _ => go E
+  | H: sub_typ ?E _ T |- _ => go E
+  end : core.
+
+#[export] Hint Extern 1 (shape ?T) =>
+  let go E := apply (shape_from_wf_shp E); auto in
+  match goal with
+  | H: typing ?E _ (pair T _) |- _ => go E
+  | H: sub_shp ?E T _ |- _ => go E 
+  | H: sub_shp ?E _ T |- _ => go E
+  end : core.
+
+#[export] Hint Extern 1 (capture ?T) =>
+  let go E := apply (capture_from_wf_cap E); auto in
+  match goal with
+  | H: typing ?E _ (pair _ T) |- _ => go E
+  | H: sub_cap ?E T _ |- _ => go E
+  | H: sub_cap ?E _ T |- _ => go E
   end : core.
 
 #[export] Hint Extern 1 (expr ?e) =>
@@ -419,3 +1797,5 @@ Qed.
   | H: red ?e _ |- _ => apply (proj1 (red_regular _ _ H))
   | H: red _ ?e |- _ => apply (proj2 (red_regular _ _ H))
   end : core.
+
+#[export] Hint Resolve wf_shp_from_wf_typ wf_cap_from_wf_typ : core.
